introduce hpsim_specC

proofmode/HPSim.v
@@ -15,7 +15,7 @@ Require Import RelationPairs.
 
 From ExtLib Require Import
      Data.Map.FMapAList.
-		 
+     
 Require Import Red IRed.
 
 Require Import ProofMode Invariant.
@@ -29,7 +29,7 @@ Section SIM.
   Variable fl_src: alist gname (Any.t -> itree hAGEs Any.t).
   Variable fl_tgt: alist gname (Any.t -> itree hAGEs Any.t).
   Variable I: Any.t -> Any.t -> iProp.
-	
+  
   Inductive _hpsim {with_dummy: bool}
     (hpsim: forall R (RR: Any.t * R -> Any.t * R -> iProp), bool -> bool -> Any.t * itree hAGEs R -> Any.t * itree hAGEs R -> Σ -> Prop)
     {R} {RR: Any.t * R -> Any.t * R -> iProp}: bool -> bool -> Any.t * itree hAGEs R -> Any.t * itree hAGEs R -> Σ -> Prop :=
@@ -45,16 +45,16 @@ Section SIM.
       fn varg k_src k_tgt FR
       (INV: Own fmr ⊢ #=> (I st_src st_tgt ** FR))
       (K: forall vret st_src0 st_tgt0 fmr0 
-		 (WF: URA.wf fmr0)
+     (WF: URA.wf fmr0)
                  (INV: Own fmr0 ⊢ #=> (I st_src0 st_tgt0 ** FR)),
-	  _hpsim hpsim true true (st_src0, k_src vret) (st_tgt0, k_tgt vret) fmr0)				
+    _hpsim hpsim true true (st_src0, k_src vret) (st_tgt0, k_tgt vret) fmr0)				
     :
     _hpsim hpsim p_src p_tgt (st_src, trigger (Call fn varg) >>= k_src) (st_tgt, trigger (Call fn varg) >>= k_tgt) fmr
   | hpsim_syscall
       p_src p_tgt st_src st_tgt fmr
       fn varg rvs k_src k_tgt
       (K: forall vret, 
-	  _hpsim hpsim true true (st_src, k_src vret) (st_tgt, k_tgt vret) fmr)
+    _hpsim hpsim true true (st_src, k_src vret) (st_tgt, k_tgt vret) fmr)
     :
     _hpsim hpsim p_src p_tgt (st_src, trigger (Syscall fn varg rvs) >>= k_src) (st_tgt, trigger (Syscall fn varg rvs) >>= k_tgt) fmr
 
@@ -221,7 +221,372 @@ Section SIM.
     pstep. eapply _hpsim_mon_progress; eauto.
     eapply paco7_mon_bot in SIM; eauto. punfold SIM.
   Qed.
-                
+
+  Variant hpsim_specC {with_dummy: bool}
+  (hpsim: forall R (RR: Any.t * R -> Any.t * R -> iProp), bool -> bool -> Any.t * itree hAGEs R -> Any.t * itree hAGEs R -> Σ -> Prop)
+  {R} {RR: Any.t * R -> Any.t * R -> iProp}: bool -> bool -> Any.t * itree hAGEs R -> Any.t * itree hAGEs R -> Σ -> Prop :=
+  | hpsim_specC_ret
+      p_src p_tgt st_src st_tgt fmr
+      v_src v_tgt
+      (* Note: (INV: Own fmr ⊢ #=> I st_src st_tgt) is required only for the funtion end. *)
+      (RET: Own fmr ⊢ #=> RR (st_src,v_src) (st_tgt,v_tgt))
+    :
+      hpsim_specC hpsim p_src p_tgt (st_src, Ret v_src) (st_tgt, Ret v_tgt) fmr
+  | hpsim_specC_call
+      p_src p_tgt st_src st_tgt fmr
+      fn varg k_src k_tgt FR
+      (INV: Own fmr ⊢ #=> (I st_src st_tgt ** FR))
+      (K: forall vret st_src0 st_tgt0 fmr0 
+          (WF: URA.wf fmr0)
+          (INV: Own fmr0 ⊢ #=> (I st_src0 st_tgt0 ** FR)),
+          hpsim _ RR true true (st_src0, k_src vret) (st_tgt0, k_tgt vret) fmr0)				
+    :
+      hpsim_specC hpsim p_src p_tgt (st_src, trigger (Call fn varg) >>= k_src) (st_tgt, trigger (Call fn varg) >>= k_tgt) fmr
+  | hpsim_specC_syscall
+      p_src p_tgt st_src st_tgt fmr
+      fn varg rvs k_src k_tgt
+      (K: forall vret, 
+          hpsim _ RR true true (st_src, k_src vret) (st_tgt, k_tgt vret) fmr)
+    :
+      hpsim_specC hpsim p_src p_tgt (st_src, trigger (Syscall fn varg rvs) >>= k_src) (st_tgt, trigger (Syscall fn varg rvs) >>= k_tgt) fmr
+
+  | hpsim_specC_inline_src
+      p_src p_tgt st_src st_tgt fmr
+      fn f varg k_src i_tgt
+      (FUN: alist_find fn fl_src = Some f)
+      (K: hpsim _ RR true p_tgt (st_src, f varg >>= (if with_dummy then (fun x => trigger (Guarantee True) ;;; k_src x) else k_src)) (st_tgt, i_tgt) fmr)
+    :
+      hpsim_specC hpsim p_src p_tgt (st_src, trigger (Call fn varg) >>= k_src) (st_tgt, i_tgt) fmr
+
+  | hpsim_specC_inline_tgt
+      p_src p_tgt st_src st_tgt fmr
+      fn f varg i_src k_tgt
+      (FUN: alist_find fn fl_tgt = Some f)
+      (K: hpsim _ RR p_src true (st_src, i_src) (st_tgt, f varg >>= (if with_dummy then (fun x => trigger (Guarantee True) ;;; k_tgt x) else k_tgt)) fmr)
+    :
+      hpsim_specC hpsim p_src p_tgt (st_src, i_src) (st_tgt, trigger (Call fn varg) >>= k_tgt) fmr
+
+  | hpsim_specC_tau_src
+      p_src p_tgt st_src st_tgt fmr
+      i_src i_tgt
+      (K: hpsim _ RR true p_tgt (st_src, i_src) (st_tgt, i_tgt) fmr)
+    :
+      hpsim_specC hpsim p_src p_tgt (st_src, tau;; i_src) (st_tgt, i_tgt) fmr
+
+  | hpsim_specC_tau_tgt
+      p_src p_tgt st_src st_tgt fmr
+      i_src i_tgt
+      (K: hpsim _ RR p_src true (st_src, i_src) (st_tgt, i_tgt) fmr)
+    :
+      hpsim_specC hpsim p_src p_tgt (st_src, i_src) (st_tgt, tau;; i_tgt) fmr
+
+  | hpsim_specC_choose_src
+      p_src p_tgt st_src st_tgt fmr
+      X x k_src i_tgt
+      (K: hpsim _ RR true p_tgt (st_src, k_src x) (st_tgt, i_tgt) fmr)
+    :
+       hpsim_specC hpsim p_src p_tgt (st_src, trigger (Choose X) >>= k_src) (st_tgt, i_tgt) fmr
+
+  | hpsim_specC_choose_tgt
+      p_src p_tgt st_src st_tgt fmr
+      X i_src k_tgt
+      (K: forall (x: X), hpsim _ RR p_src true (st_src, i_src) (st_tgt, k_tgt x) fmr)
+    :
+      hpsim_specC hpsim p_src p_tgt (st_src, i_src) (st_tgt, trigger (Choose X) >>= k_tgt) fmr
+
+  | hpsim_specC_take_src
+      p_src p_tgt st_src st_tgt fmr
+      X k_src i_tgt
+      (K: forall (x: X), hpsim _ RR true p_tgt (st_src, k_src x) (st_tgt, i_tgt) fmr)
+    :
+      hpsim_specC hpsim p_src p_tgt (st_src, trigger (Take X) >>= k_src) (st_tgt, i_tgt) fmr
+
+  | hpsim_specC_take_tgt
+      p_src p_tgt st_src st_tgt fmr
+      X x i_src k_tgt
+      (K: hpsim _ RR p_src true (st_src, i_src) (st_tgt, k_tgt x) fmr)
+    :
+      hpsim_specC hpsim p_src p_tgt (st_src, i_src) (st_tgt, trigger (Take X) >>= k_tgt) fmr
+
+  | hpsim_specC_supdate_src
+      p_src p_tgt st_src st_tgt fmr
+      X x st_src0 k_src i_tgt
+      (run: Any.t -> Any.t * X)
+      (RUN: run st_src = (st_src0, x))
+      (K: hpsim _ RR true p_tgt (st_src0, k_src x) (st_tgt, i_tgt) fmr)
+    :
+      hpsim_specC hpsim p_src p_tgt (st_src, trigger (SUpdate run) >>= k_src) (st_tgt, i_tgt) fmr
+
+  | hpsim_specC_supdate_tgt
+      p_src p_tgt st_src st_tgt fmr
+      X x st_tgt0 i_src k_tgt
+      (run: Any.t -> Any.t * X)
+      (RUN: run st_tgt = (st_tgt0, x))
+      (K: hpsim _ RR p_src true (st_src, i_src) (st_tgt0, k_tgt x) fmr)
+    :
+      hpsim_specC hpsim p_src p_tgt (st_src, i_src) (st_tgt, trigger (SUpdate run) >>= k_tgt) fmr
+
+  | hpsim_specC_assume_src
+      p_src p_tgt st_src st_tgt fmr
+      iP k_src i_tgt FMR
+      (CUR: Own fmr ⊢ #=> FMR)
+      (K: forall fmr0 (WF: URA.wf fmr0) (NEW: Own fmr0 ⊢ #=> (iP ** FMR)),
+          hpsim _ RR true p_tgt (st_src, k_src tt) (st_tgt, i_tgt) fmr0)
+    :
+      hpsim_specC hpsim p_src p_tgt (st_src, trigger (Assume iP) >>= k_src) (st_tgt, i_tgt) fmr
+
+  | hpsim_specC_assume_tgt
+      p_src p_tgt st_src st_tgt fmr
+      iP i_src k_tgt FMR
+      (CUR: Own fmr ⊢ #=> (iP ** FMR))
+      (K: forall fmr0 (WF: URA.wf fmr0) (NEW: Own fmr0 ⊢ #=> FMR),
+          hpsim _ RR p_src true (st_src, i_src) (st_tgt, k_tgt tt) fmr0)
+    :
+      hpsim_specC hpsim p_src p_tgt (st_src, i_src) (st_tgt, trigger (Assume iP) >>= k_tgt) fmr
+
+  | hpsim_specC_guarantee_src
+      p_src p_tgt st_src st_tgt fmr
+      iP k_src i_tgt FMR
+      (CUR: Own fmr ⊢ #=> (iP ** FMR))
+      (K: forall fmr0 (WF: URA.wf fmr0) (NEW: Own fmr0 ⊢ #=> FMR),
+          hpsim _ RR true p_tgt (st_src, k_src tt) (st_tgt, i_tgt) fmr0)
+    :
+      hpsim_specC hpsim p_src p_tgt (st_src, trigger (Guarantee iP) >>= k_src) (st_tgt, i_tgt) fmr
+
+  | hpsim_specC_guarantee_tgt
+      p_src p_tgt st_src st_tgt fmr
+      iP i_src k_tgt FMR
+      (CUR: Own fmr ⊢ #=> FMR)
+      (K: forall fmr0 (WF: URA.wf fmr0) (NEW: Own fmr0 ⊢ #=> (iP ** FMR)),
+          hpsim _ RR p_src true (st_src, i_src) (st_tgt, k_tgt tt) fmr0)
+    :
+      hpsim_specC hpsim p_src p_tgt (st_src, i_src) (st_tgt, trigger (Guarantee iP) >>= k_tgt) fmr
+  .
+  
+  Lemma hpsim_specC_mon with_dummy : monotone7 (@hpsim_specC with_dummy).
+  Proof.
+    ii. inv IN; try (by des; econs; ss; et).
+  Qed.
+
+  Hint Resolve hpsim_specC_mon: paco.
+
+  Lemma hpsim_specC_spec with_dummy:
+    (@hpsim_specC with_dummy) <8= gupaco7 (@_hpsim with_dummy) (cpn7 (@_hpsim with_dummy)).
+  Proof.
+    eapply wrespect7_uclo; eauto with paco.
+    econs; eauto with paco; i.
+    inv PR; econs; et; try (i; eapply _hpsim_mon; et; i; eapply rclo7_base; et).
+  Qed.
+  
+  Variant hpsimC {with_dummy: bool}
+  (r g: forall R (RR: Any.t * R -> Any.t * R -> iProp), bool -> bool -> Any.t * itree hAGEs R -> Any.t * itree hAGEs R -> Σ -> Prop)
+  {R} {RR: Any.t * R -> Any.t * R -> iProp}: bool -> bool -> Any.t * itree hAGEs R -> Any.t * itree hAGEs R -> Σ -> Prop :=
+  | hpsimC_ret
+      p_src p_tgt st_src st_tgt fmr
+      v_src v_tgt
+      (RET: Own fmr ⊢ #=> RR (st_src,v_src) (st_tgt,v_tgt))
+    :
+      hpsimC r g p_src p_tgt (st_src, Ret v_src) (st_tgt, Ret v_tgt) fmr
+  | hpsimC_call
+      p_src p_tgt st_src st_tgt fmr
+      fn varg k_src k_tgt FR
+      (INV: Own fmr ⊢ #=> (I st_src st_tgt ** FR))
+      (K: forall vret st_src0 st_tgt0 fmr0 
+          (WF: URA.wf fmr0)
+          (INV: Own fmr0 ⊢ #=> (I st_src0 st_tgt0 ** FR)),
+          r _ RR true true (st_src0, k_src vret) (st_tgt0, k_tgt vret) fmr0)				
+    :
+      hpsimC r g p_src p_tgt (st_src, trigger (Call fn varg) >>= k_src) (st_tgt, trigger (Call fn varg) >>= k_tgt) fmr
+  | hpsimC_syscall
+      p_src p_tgt st_src st_tgt fmr
+      fn varg rvs k_src k_tgt
+      (K: forall vret, 
+          r _ RR true true (st_src, k_src vret) (st_tgt, k_tgt vret) fmr)
+    :
+      hpsimC r g p_src p_tgt (st_src, trigger (Syscall fn varg rvs) >>= k_src) (st_tgt, trigger (Syscall fn varg rvs) >>= k_tgt) fmr
+
+  | hpsimC_inline_src
+      p_src p_tgt st_src st_tgt fmr
+      fn f varg k_src i_tgt
+      (FUN: alist_find fn fl_src = Some f)
+      (K: r _ RR true p_tgt (st_src, f varg >>= (if with_dummy then (fun x => trigger (Guarantee True) ;;; k_src x) else k_src)) (st_tgt, i_tgt) fmr)
+    :
+      hpsimC r g p_src p_tgt (st_src, trigger (Call fn varg) >>= k_src) (st_tgt, i_tgt) fmr
+
+  | hpsimC_inline_tgt
+      p_src p_tgt st_src st_tgt fmr
+      fn f varg i_src k_tgt
+      (FUN: alist_find fn fl_tgt = Some f)
+      (K: r _ RR p_src true (st_src, i_src) (st_tgt, f varg >>= (if with_dummy then (fun x => trigger (Guarantee True) ;;; k_tgt x) else k_tgt)) fmr)
+    :
+      hpsimC r g p_src p_tgt (st_src, i_src) (st_tgt, trigger (Call fn varg) >>= k_tgt) fmr
+
+  | hpsimC_tau_src
+      p_src p_tgt st_src st_tgt fmr
+      i_src i_tgt
+      (K: r _ RR true p_tgt (st_src, i_src) (st_tgt, i_tgt) fmr)
+    :
+      hpsimC r g p_src p_tgt (st_src, tau;; i_src) (st_tgt, i_tgt) fmr
+
+  | hpsimC_tau_tgt
+      p_src p_tgt st_src st_tgt fmr
+      i_src i_tgt
+      (K: r _ RR p_src true (st_src, i_src) (st_tgt, i_tgt) fmr)
+    :
+      hpsimC r g p_src p_tgt (st_src, i_src) (st_tgt, tau;; i_tgt) fmr
+
+  | hpsimC_choose_src
+      p_src p_tgt st_src st_tgt fmr
+      X x k_src i_tgt
+      (K: r _ RR true p_tgt (st_src, k_src x) (st_tgt, i_tgt) fmr)
+    :
+       hpsimC r g p_src p_tgt (st_src, trigger (Choose X) >>= k_src) (st_tgt, i_tgt) fmr
+
+  | hpsimC_choose_tgt
+      p_src p_tgt st_src st_tgt fmr
+      X i_src k_tgt
+      (K: forall (x: X), r _ RR p_src true (st_src, i_src) (st_tgt, k_tgt x) fmr)
+    :
+      hpsimC r g p_src p_tgt (st_src, i_src) (st_tgt, trigger (Choose X) >>= k_tgt) fmr
+
+  | hpsimC_take_src
+      p_src p_tgt st_src st_tgt fmr
+      X k_src i_tgt
+      (K: forall (x: X), r _ RR true p_tgt (st_src, k_src x) (st_tgt, i_tgt) fmr)
+    :
+      hpsimC r g p_src p_tgt (st_src, trigger (Take X) >>= k_src) (st_tgt, i_tgt) fmr
+
+  | hpsimC_take_tgt
+      p_src p_tgt st_src st_tgt fmr
+      X x i_src k_tgt
+      (K: r _ RR p_src true (st_src, i_src) (st_tgt, k_tgt x) fmr)
+    :
+      hpsimC r g p_src p_tgt (st_src, i_src) (st_tgt, trigger (Take X) >>= k_tgt) fmr
+
+  | hpsimC_supdate_src
+      p_src p_tgt st_src st_tgt fmr
+      X x st_src0 k_src i_tgt
+      (run: Any.t -> Any.t * X)
+      (RUN: run st_src = (st_src0, x))
+      (K: r _ RR true p_tgt (st_src0, k_src x) (st_tgt, i_tgt) fmr)
+    :
+      hpsimC r g p_src p_tgt (st_src, trigger (SUpdate run) >>= k_src) (st_tgt, i_tgt) fmr
+
+  | hpsimC_supdate_tgt
+      p_src p_tgt st_src st_tgt fmr
+      X x st_tgt0 i_src k_tgt
+      (run: Any.t -> Any.t * X)
+      (RUN: run st_tgt = (st_tgt0, x))
+      (K: r _ RR p_src true (st_src, i_src) (st_tgt0, k_tgt x) fmr)
+    :
+      hpsimC r g p_src p_tgt (st_src, i_src) (st_tgt, trigger (SUpdate run) >>= k_tgt) fmr
+
+  | hpsimC_assume_src
+      p_src p_tgt st_src st_tgt fmr
+      iP k_src i_tgt FMR
+      (CUR: Own fmr ⊢ #=> FMR)
+      (K: forall fmr0 (WF: URA.wf fmr0) (NEW: Own fmr0 ⊢ #=> (iP ** FMR)),
+          r _ RR true p_tgt (st_src, k_src tt) (st_tgt, i_tgt) fmr0)
+    :
+      hpsimC r g p_src p_tgt (st_src, trigger (Assume iP) >>= k_src) (st_tgt, i_tgt) fmr
+
+  | hpsimC_assume_tgt
+      p_src p_tgt st_src st_tgt fmr
+      iP i_src k_tgt FMR
+      (CUR: Own fmr ⊢ #=> (iP ** FMR))
+      (K: forall fmr0 (WF: URA.wf fmr0) (NEW: Own fmr0 ⊢ #=> FMR),
+          r _ RR p_src true (st_src, i_src) (st_tgt, k_tgt tt) fmr0)
+    :
+      hpsimC r g p_src p_tgt (st_src, i_src) (st_tgt, trigger (Assume iP) >>= k_tgt) fmr
+
+  | hpsimC_guarantee_src
+      p_src p_tgt st_src st_tgt fmr
+      iP k_src i_tgt FMR
+      (CUR: Own fmr ⊢ #=> (iP ** FMR))
+      (K: forall fmr0 (WF: URA.wf fmr0) (NEW: Own fmr0 ⊢ #=> FMR),
+          r _ RR true p_tgt (st_src, k_src tt) (st_tgt, i_tgt) fmr0)
+    :
+      hpsimC r g p_src p_tgt (st_src, trigger (Guarantee iP) >>= k_src) (st_tgt, i_tgt) fmr
+
+  | hpsimC_guarantee_tgt
+      p_src p_tgt st_src st_tgt fmr
+      iP i_src k_tgt FMR
+      (CUR: Own fmr ⊢ #=> FMR)
+      (K: forall fmr0 (WF: URA.wf fmr0) (NEW: Own fmr0 ⊢ #=> (iP ** FMR)),
+          r _ RR p_src true (st_src, i_src) (st_tgt, k_tgt tt) fmr0)
+    :
+      hpsimC r g p_src p_tgt (st_src, i_src) (st_tgt, trigger (Guarantee iP) >>= k_tgt) fmr
+  .
+  
+  Lemma hpsimC_spec with_dummy r g:
+    (@hpsimC with_dummy) (gpaco7 (@_hpsim with_dummy) (cpn7 (@_hpsim with_dummy)) r g) (gpaco7 (@_hpsim with_dummy) (cpn7 (@_hpsim with_dummy)) g g)
+    <7=
+    gpaco7 (@_hpsim with_dummy) (cpn7 (@_hpsim with_dummy)) r g.
+  Proof.
+    i. eapply gpaco7_gpaco; [eauto with paco|].
+    eapply gpaco7_mon; [|eauto|i; eapply gupaco7_mon; et].
+    inv PR; try (guclo hpsim_specC_spec; econs; et; i; gbase; et).
+  Qed.
+
+  Lemma hpsim_progress_flag with_dummy R RR r g st_src st_tgt fmr
+        (SIM: gpaco7 (@_hpsim with_dummy) (cpn7 (@_hpsim with_dummy)) g g R RR false false st_src st_tgt fmr)
+      :
+        gpaco7 (@_hpsim with_dummy) (cpn7 (@_hpsim with_dummy)) r g R RR true true st_src st_tgt fmr.
+  Proof.
+    gstep. destruct st_src, st_tgt. econs; et.
+  Qed.
+
+  Lemma hpsim_flag_mon with_dummy
+        (hpsim: forall (R: Type) (RR: Any.t * R -> Any.t * R -> iProp),  bool -> bool -> Any.t * itree hAGEs R -> Any.t * itree hAGEs R -> Σ -> Prop)
+        R (RR: Any.t * R -> Any.t * R -> iProp)
+        p_src0 p_tgt0 p_src1 p_tgt1 st_src st_tgt fmr
+        (SIM: (@_hpsim with_dummy) hpsim _ RR p_src0 p_tgt0 st_src st_tgt fmr)
+        (SRC: p_src0 = true -> p_src1 = true)
+        (TGT: p_tgt0 = true -> p_tgt1 = true)
+    :
+        (@_hpsim with_dummy) hpsim _ RR p_src1 p_tgt1 st_src st_tgt fmr.
+  Proof.
+    revert p_src1 p_tgt1 SRC TGT.
+    induction SIM; i; clarify; et.
+    exploit SRC; et. exploit TGT; et. i. clarify. econs; et.
+  Qed.              
+
+  Variant hpsim_flagC 
+    (r: forall (R: Type) (RR: Any.t * R -> Any.t * R -> iProp),  bool -> bool -> Any.t * itree hAGEs R -> Any.t * itree hAGEs R -> Σ -> Prop)
+    {R} (RR: Any.t * R -> Any.t * R -> iProp): bool -> bool -> Any.t * itree hAGEs R -> Any.t * itree hAGEs R -> Σ -> Prop := 
+  | hpsim_flagC_intro
+    p_src0 p_tgt0 p_src1 p_tgt1 st_src st_tgt fmr
+    (SIM: r _ RR p_src0 p_tgt0 st_src st_tgt fmr)
+    (SRC: p_src0 = true -> p_src1 = true)
+    (TGT: p_tgt0 = true -> p_tgt1 = true)
+  :
+    hpsim_flagC r RR p_src1 p_tgt1 st_src st_tgt fmr
+  .   
+
+  Lemma hpsim_flagC_mon r1 r2 (LE: r1 <7= r2) : @hpsim_flagC r1 <7= @hpsim_flagC r2.
+  Proof. ii. destruct PR; econs; et. Qed.
+
+  Hint Resolve hpsim_flagC_mon: paco.
+  
+  Lemma hpsim_flagC_spec with_dummy: hpsim_flagC <8= gupaco7 (@_hpsim with_dummy) (cpn7 (@_hpsim with_dummy)).
+  Proof.
+    eapply wrespect7_uclo; eauto with paco.
+    econs; eauto with paco. i. inv PR.
+    eapply GF in SIM.
+    revert x2 x3 SRC TGT. induction SIM; i; clarify; et.
+    exploit SRC; et. exploit TGT; et. i. clarify. econs; et.
+    eapply rclo7_base; et.
+  Qed.
+
+  Lemma hpsim_flag_down with_dummy R RR r g p_src p_tgt st_src st_tgt fmr
+        (SIM: gpaco7 (@_hpsim with_dummy) (cpn7 (@_hpsim with_dummy)) r g R RR false false st_src st_tgt fmr)
+      :
+        gpaco7 (@_hpsim with_dummy) (cpn7 (@_hpsim with_dummy)) r g R RR p_src p_tgt st_src st_tgt fmr.
+  Proof. 
+    guclo hpsim_flagC_spec. econs; et. 
+  Qed.
+
+
   Variant hpsim_bindC (r: forall R (RR: Any.t * R -> Any.t * R -> iProp), bool -> bool -> Any.t * itree hAGEs R -> Any.t * itree hAGEs R -> Σ -> Prop):
     forall R (RR: Any.t * R -> Any.t * R -> iProp), bool -> bool -> Any.t * itree hAGEs R -> Any.t * itree hAGEs R -> Σ -> Prop
   :=
@@ -303,135 +668,135 @@ Section SIM.
     @hpsim <7= paco7 (@_hpsim true) bot7.
   Proof. ginit. eauto with paco. Qed.
                 
-	Lemma current_iProp_sepconj P Q r 
-			(SAT: current_iProp r (P ** Q))
-		:
-			exists rp rq, URA.updatable r (rp ⋅ rq) /\ current_iProp rp P /\ current_iProp rq Q
-	.
-	Proof.
-		destruct SAT. rr in IPROP. uipropall. des. clarify.
-		hexploit UPD. i. eapply URA.updatable_wf in H; et. des.
-		esplits; et; econs; et; r_solve.
-		- eapply URA.wf_mon in H. et.
-		- eapply URA.wf_extends in H; et. econs. instantiate (1:= a). r_solve.
-	Qed.
+  Lemma current_iProp_sepconj P Q r 
+      (SAT: current_iProp r (P ** Q))
+    :
+      exists rp rq, URA.updatable r (rp ⋅ rq) /\ current_iProp rp P /\ current_iProp rq Q
+  .
+  Proof.
+    destruct SAT. rr in IPROP. uipropall. des. clarify.
+    hexploit UPD. i. eapply URA.updatable_wf in H; et. des.
+    esplits; et; econs; et; r_solve.
+    - eapply URA.wf_mon in H. et.
+    - eapply URA.wf_extends in H; et. econs. instantiate (1:= a). r_solve.
+  Qed.
 
-	Lemma own_ctx a b
-			(OWN: Own a ⊢ #=> Own b)
-		:
-			forall ctx, Own (ctx ⋅ a) ⊢ #=> Own (ctx ⋅ b)
-	.
-	Proof.
-		i. iIntros "[H H0]".
-		iPoseProof (OWN with "H0") as "H0".
-		iSplitL "H"; et.
-	Qed.
+  Lemma own_ctx a b
+      (OWN: Own a ⊢ #=> Own b)
+    :
+      forall ctx, Own (ctx ⋅ a) ⊢ #=> Own (ctx ⋅ b)
+  .
+  Proof.
+    i. iIntros "[H H0]".
+    iPoseProof (OWN with "H0") as "H0".
+    iSplitL "H"; et.
+  Qed.
 
-	Lemma own_wf (r r': Σ)
-			(OWN: Own r ⊢ #=> Own r')
-			(WF: URA.wf r)
-		:
-			URA.wf r'
-	.
-	Proof. 
-		uipropall. hexploit OWN; et. refl.
-		esplits; et. des.
-		eapply URA.wf_extends; et.
-		specialize (H0 ε). rewrite ! URA.unit_id in H0.
-		et.
-	Qed.
+  Lemma own_wf (r r': Σ)
+      (OWN: Own r ⊢ #=> Own r')
+      (WF: URA.wf r)
+    :
+      URA.wf r'
+  .
+  Proof. 
+    uipropall. hexploit OWN; et. refl.
+    esplits; et. des.
+    eapply URA.wf_extends; et.
+    specialize (H0 ε). rewrite ! URA.unit_id in H0.
+    et.
+  Qed.
 
 
 
-	Lemma not_wf_sat (r: Σ) (ILL: ¬ URA.wf r) P: Own r ⊢ P.
-	Proof.
-		rr. uipropall. i.
-		eapply URA.wf_extends in WF; et.
-		clarify.
-	Qed.
+  Lemma not_wf_sat (r: Σ) (ILL: ¬ URA.wf r) P: Own r ⊢ P.
+  Proof.
+    rr. uipropall. i.
+    eapply URA.wf_extends in WF; et.
+    clarify.
+  Qed.
 
-	Lemma iProp_sepconj_aux P Q r 
-			(SAT: Own r ⊢ #=> (P ** Q))
-		:
-			exists rp rq, (URA.updatable r (rp ⋅ rq)) /\ 
-										(Own rp ⊢ P) /\ 
-										(Own rq ⊢ Q)
-	.
-	Proof.
-		destruct (classic (URA.wf r)); cycle 1.
-		{
-			exists r, r. esplits; eauto using not_wf_sat.
-			rr. i. eapply URA.wf_mon in H0. clarify. 
-		}
+  Lemma iProp_sepconj_aux P Q r 
+      (SAT: Own r ⊢ #=> (P ** Q))
+    :
+      exists rp rq, (URA.updatable r (rp ⋅ rq)) /\ 
+                    (Own rp ⊢ P) /\ 
+                    (Own rq ⊢ Q)
+  .
+  Proof.
+    destruct (classic (URA.wf r)); cycle 1.
+    {
+      exists r, r. esplits; eauto using not_wf_sat.
+      rr. i. eapply URA.wf_mon in H0. clarify. 
+    }
 
-		uipropall.
-		hexploit SAT; et. { r_solve. }
-		i. des.
-		esplits; et; uipropall.
-		{
-			instantiate (1:= b). instantiate (1:=a).
-			unfold URA.updatable. subst. et. 
-		}
-		{
-			i. destruct P. ss.
-			hexploit H4. i.
-			eapply URA.wf_extends in H4; et.
-		}
-		{
-			i. destruct Q. ss.
-			hexploit H4. i.
-			eapply URA.wf_extends in H4; et.
-		}
-	Qed.
+    uipropall.
+    hexploit SAT; et. { r_solve. }
+    i. des.
+    esplits; et; uipropall.
+    {
+      instantiate (1:= b). instantiate (1:=a).
+      unfold URA.updatable. subst. et. 
+    }
+    {
+      i. destruct P. ss.
+      hexploit H4. i.
+      eapply URA.wf_extends in H4; et.
+    }
+    {
+      i. destruct Q. ss.
+      hexploit H4. i.
+      eapply URA.wf_extends in H4; et.
+    }
+  Qed.
 
-	Lemma iProp_sepconj P Q r 
-			(SAT: Own r ⊢ #=> (P ** Q))
-		:
-			exists rp rq, (Own r ⊢ #=> Own (rp ⋅ rq)) /\ 
-										(Own rp ⊢ P) /\ 
-										(Own rq ⊢ Q)
-	.
-	Proof.
-		eapply iProp_sepconj_aux in SAT; et. des.
-		eapply Own_Upd in SAT.
-		esplits; et. 	
-	Qed.	
+  Lemma iProp_sepconj P Q r 
+      (SAT: Own r ⊢ #=> (P ** Q))
+    :
+      exists rp rq, (Own r ⊢ #=> Own (rp ⋅ rq)) /\ 
+                    (Own rp ⊢ P) /\ 
+                    (Own rq ⊢ Q)
+  .
+  Proof.
+    eapply iProp_sepconj_aux in SAT; et. des.
+    eapply Own_Upd in SAT.
+    esplits; et. 	
+  Qed.	
 
-	Lemma current_iProp_sepconj' P Q r 
-			(SAT: current_iProp r (P ** Q))
-		:
-			exists rp rq, URA.updatable r (rp ⋅ rq) /\ P rp /\ Q rq
-	.
-	Proof.
-		destruct SAT. rr in IPROP. uipropall. des. clarify.
-		hexploit UPD. i. eapply URA.updatable_wf in H; et. 
-	Qed.
+  Lemma current_iProp_sepconj' P Q r 
+      (SAT: current_iProp r (P ** Q))
+    :
+      exists rp rq, URA.updatable r (rp ⋅ rq) /\ P rp /\ Q rq
+  .
+  Proof.
+    destruct SAT. rr in IPROP. uipropall. des. clarify.
+    hexploit UPD. i. eapply URA.updatable_wf in H; et. 
+  Qed.
 
-	Lemma current_iProp_sepconj_r P Q r 
-			(SAT: current_iProp r (P ** Q))
-		:
-			exists rp rq, URA.updatable r (rp ⋅ rq) /\ P rp /\ current_iProp rq Q
-	.
-	Proof.
-		destruct SAT. rr in IPROP. uipropall. des. clarify.
-		hexploit UPD. i. eapply URA.updatable_wf in H; et. 
-		esplits; et; econs; et; r_solve.
-		des. eapply URA.wf_extends; et. econs. instantiate (1:= a). r_solve.
-	Qed.
+  Lemma current_iProp_sepconj_r P Q r 
+      (SAT: current_iProp r (P ** Q))
+    :
+      exists rp rq, URA.updatable r (rp ⋅ rq) /\ P rp /\ current_iProp rq Q
+  .
+  Proof.
+    destruct SAT. rr in IPROP. uipropall. des. clarify.
+    hexploit UPD. i. eapply URA.updatable_wf in H; et. 
+    esplits; et; econs; et; r_solve.
+    des. eapply URA.wf_extends; et. econs. instantiate (1:= a). r_solve.
+  Qed.
 
-	Lemma current_iProp_conj P Q x y
-			(IP: current_iProp x P)
-			(IQ: current_iProp y Q)
-			(WF: URA.wf (x ⋅ y))
-	:
-			current_iProp (x ⋅ y) (P ** Q)
-	.
-	Proof. 
-		inv IP. inv IQ.
-		econs; et.
-		{ uipropall. esplits; et. }
-		eapply URA.updatable_add; et.
-	Qed.
+  Lemma current_iProp_conj P Q x y
+      (IP: current_iProp x P)
+      (IQ: current_iProp y Q)
+      (WF: URA.wf (x ⋅ y))
+  :
+      current_iProp (x ⋅ y) (P ** Q)
+  .
+  Proof. 
+    inv IP. inv IQ.
+    econs; et.
+    { uipropall. esplits; et. }
+    eapply URA.updatable_add; et.
+  Qed.
 
 
   Lemma current_iPropL_convert fmr P
@@ -1195,6 +1560,7 @@ Section SIM.
     | interp_inv_intro
         (ctx mr_src mr_tgt: Σ) st_src st_tgt mr
         (WF: URA.wf (ctx ⋅ mr_src))
+        (* (MRS: Own (ctx ⋅ mr_src) ⊢ #=> Own (ctx ⋅ mr ⋅ mr_tgt)) *)
         (MRS: Own mr_src ⊢ #=> Own (mr ⋅ mr_tgt))
         (MR: Own mr ⊢ #=> I st_src st_tgt)
       :
@@ -1220,8 +1586,54 @@ Section SIM.
     remember (st_src, itr_src). remember (st_tgt, itr_tgt).
     move SIM before FLT. revert_until SIM.
     punfold SIM. induction SIM; i; clarify.
-    - admit.
-    - admit.
+    - unfold interp_hp_body, hp_fun_tail, handle_Guarantee, guarantee, mget, mput.
+      steps. force_l. instantiate (1 := (c0 ⋅ c1, ε, fmr ⋅ c)). steps.
+      force_l.
+      { 
+        rewrite FMR. 
+        iIntros "H". iMod "H".
+        rewrite <- URA.add_assoc. 
+        iDestruct "H" as "[H H0]".
+        iPoseProof (x with "H0") as "H0".
+        iMod "H0".
+        iModIntro. r_solve.
+        iDestruct "H0" as "[H0 H1]".
+        iSplitR "H1"; et.
+        iCombine "H0 H" as "H". et.
+      } 
+      steps. force_l. 
+      { iIntros "H". et. } 
+      steps. econs. esplits; et. econs; esplits; et.
+      instantiate (1:= ctx).
+      {
+        eapply own_ctx in FMR, x. rewrite URA.add_assoc in FMR. eapply own_wf in FMR; et.
+        rewrite <- URA.add_assoc in FMR. rewrite URA.add_assoc in FMR.
+        eapply own_wf in x; et.
+        replace (ctx ⋅ fmr ⋅ (c0 ⋅ c1 ⋅ c)) with (ctx ⋅ fmr ⋅ c ⋅ (c0 ⋅ c1)) in x; r_solve.
+        eapply URA.wf_mon; et.
+      }.
+    - unfold interp_hp_body, hp_fun_tail, handle_Guarantee, mget, mput, guarantee.
+      hexploit INV. i.
+      eapply iProp_sepconj in H0; et. des. rename rq into fr. rename rp into mr.
+      steps. unfold handle_Guarantee, guarantee, mget, mput. steps_safe.
+      (* force_l. instantiate (1:= (ε, fr_src, mr_src)). steps_safe. *)
+      force_l. instantiate (1:= (c0, fr ⋅ c1, mr ⋅ c)). steps_safe.
+      rename c1 into frt. rename c into mrt.
+      force_l.
+      { admit. }
+      steps_safe. 
+      force_l; et.
+      steps_safe. eapply safe_sim_sim; econs. esplits; i.
+      { 
+        econs.
+        { instantiate (1:= ctx ⋅ fr ⋅ frt). admit. }
+        { instantiate (1:= mr). admit. }
+        { admit. }
+      }
+      steps.
+      inv WF0. eapply H; [| |et|et| |].
+      (* expect w1 = ctx ⋅ fr ⋅ frt *)
+      all: admit.
     - admit.
     - exploit IHSIM; eauto. i.
       rewrite-> interp_hp_body_bind, interp_hp_call.
@@ -1230,7 +1642,7 @@ Section SIM.
       steps. force_l. { r_solve; et. }
       steps. force_l; et. steps.
       {	instantiate (1:= interp_hp_fun f).
-	rewrite alist_find_map. rewrite FUN. et. }
+  rewrite alist_find_map. rewrite FUN. et. }
       guclo sim_strictC_spec. econs; eauto.
       + apply interp_strict_inline_src.
       + apply sim_strict_refl.
@@ -1239,7 +1651,7 @@ Section SIM.
       unfold handle_Guarantee, mget, mput, guarantee.
       steps.
       {	instantiate (1:= interp_hp_fun f).
-	rewrite alist_find_map. rewrite FUN. et. }
+  rewrite alist_find_map. rewrite FUN. et. }
       guclo sim_strictC_spec. econs; eauto.
       + apply sim_strict_refl.      
       + apply interp_strict_inline_tgt.
@@ -1264,656 +1676,656 @@ Section SIM.
       
       
       rewrite !bind_bind. 
-		unfold interp_hp_fun.
-		gclo. eapply compatible'8_companion; eauto with paco.
-		{ eapply compat8_compatible'. apply inlineSrcC_compatible. }	
-		econs. { grind. }
-		specialize (IHSIM st_src0 st_tgt0 ((f varg) >>= k_src) itr_tgt ctx (fr_src ⋅ mr_src) mr_tgt ε fr_tgt).
-		rewrite interp_hp_fun_bind in IHSIM.
-		rewrite bind_bind in IHSIM.
-		(* unfold interp_hp_fun in IHSIM. *)
-		eapply IHSIM; r_solve; et.
-	}
+    unfold interp_hp_fun.
+    gclo. eapply compatible'8_companion; eauto with paco.
+    { eapply compat8_compatible'. apply inlineSrcC_compatible. }	
+    econs. { grind. }
+    specialize (IHSIM st_src0 st_tgt0 ((f varg) >>= k_src) itr_tgt ctx (fr_src ⋅ mr_src) mr_tgt ε fr_tgt).
+    rewrite interp_hp_fun_bind in IHSIM.
+    rewrite bind_bind in IHSIM.
+    (* unfold interp_hp_fun in IHSIM. *)
+    eapply IHSIM; r_solve; et.
+  }
 
 
 
-	- unfold interp_hp_fun, handle_Guarantee, mget, mput, guarantee.
-		steps.
-		force_l. instantiate (1 := (c0 ⋅ c1, ε, fmr ⋅ c)). steps.
-		unfold guarantee. force_l.
-		{ 
-			rewrite FMR. 
-			iIntros "H". iMod "H".
-			rewrite <- URA.add_assoc. 
-			iDestruct "H" as "[H H0]".
-			iPoseProof (x with "H0") as "H0".
-			iMod "H0".
-			iModIntro. r_solve.
-			iDestruct "H0" as "[H0 H1]".
-			iSplitR "H1"; et.
-			iCombine "H0 H" as "H". et.
-		} 
-		steps. force_l. 
-		{ iIntros "H". et. } 
-		(* rr. uipropall. }  *)
-		steps. econs. esplits; et. econs. esplits; et.
-		instantiate (1:= ctx).
-		{
-			eapply own_ctx in FMR, x. rewrite URA.add_assoc in FMR. eapply own_wf in FMR; et.
-			rewrite <- URA.add_assoc in FMR. rewrite URA.add_assoc in FMR.
-			eapply own_wf in x; et.
-			replace (ctx ⋅ fmr ⋅ (c0 ⋅ c1 ⋅ c)) with (ctx ⋅ fmr ⋅ c ⋅ (c0 ⋅ c1)) in x; r_solve.
-			eapply URA.wf_mon; et.
-		}
+  - unfold interp_hp_fun, handle_Guarantee, mget, mput, guarantee.
+    steps.
+    force_l. instantiate (1 := (c0 ⋅ c1, ε, fmr ⋅ c)). steps.
+    unfold guarantee. force_l.
+    { 
+      rewrite FMR. 
+      iIntros "H". iMod "H".
+      rewrite <- URA.add_assoc. 
+      iDestruct "H" as "[H H0]".
+      iPoseProof (x with "H0") as "H0".
+      iMod "H0".
+      iModIntro. r_solve.
+      iDestruct "H0" as "[H0 H1]".
+      iSplitR "H1"; et.
+      iCombine "H0 H" as "H". et.
+    } 
+    steps. force_l. 
+    { iIntros "H". et. } 
+    (* rr. uipropall. }  *)
+    steps. econs. esplits; et. econs. esplits; et.
+    instantiate (1:= ctx).
+    {
+      eapply own_ctx in FMR, x. rewrite URA.add_assoc in FMR. eapply own_wf in FMR; et.
+      rewrite <- URA.add_assoc in FMR. rewrite URA.add_assoc in FMR.
+      eapply own_wf in x; et.
+      replace (ctx ⋅ fmr ⋅ (c0 ⋅ c1 ⋅ c)) with (ctx ⋅ fmr ⋅ c ⋅ (c0 ⋅ c1)) in x; r_solve.
+      eapply URA.wf_mon; et.
+    }
 
-	- unfold interp_hp_fun, handle_Guarantee, mget, mput, guarantee.
-		hexploit INV. i.
-		eapply iProp_sepconj in H; et. 
-		(* 2: { admit. } *)
-		des.
-		rename rq into fr. rename rp into mr.
-		steps.
-		unfold handle_Guarantee, mget, mput. steps_safe.
-		force_l.
-		instantiate (1:= (c0, ε, fr ⋅ c1 ⋅ mr ⋅ c)).
-		steps_safe.
-		unfold guarantee. force_l.
-		{ admit. }
-			(* iIntros "H". iPoseProof (FMR with "H") as "H". iMod "H".
-			rewrite <- URA.add_assoc.
-			iDestruct "H" as "[H H0]". 
-			iPoseProof (H with "H") as "H".
-			replace (c0 ⋅ (fr ⋅ c1) ⋅ (mr ⋅ c)) with (mr ⋅ fr ⋅ (c0 ⋅ c1 ⋅ c)). 2: { r_solve. }
-			iPoseProof (_GUARANTEE with "H0") as "H0".
-			iSplitL "H"; et. *)
-		steps_safe. force_l.
-		{ et. }
-		steps_safe. eapply safe_sim_sim; econs; esplits; i.
-		{ 
-			econs. esplits; et.
-			{ instantiate (1:= ctx). admit. }
-			{ admit. }
-			(* { iIntros "H". iPoseProof (H0 with "H") as "H". et. } *)
-		}
-		inv WF0. des.
-		unfold interp_hp_fun, handle_Guarantee, mget, mput, guarantee in K.
-		steps.
-		hexploit K; swap 1 2. 
-		{ 
-			instantiate (1:= st_tgt). instantiate (1:= st_src).
-			iIntros "[H1 H2]".
-			iPoseProof (H1 with "H1") as "H1". 
-			iPoseProof (MR with "H2") as "H2".
-			iSplitL "H2"; et.
-		}
-		{ admit. }
-		i. des.
-		unfold interp_hp_fun, handle_Guarantee, mget, mput in *. rewrite <- ! bind_bind in *.
-		eapply IH; et.
-		{
-			
-		}
-	- steps. hexploit K; et. i. des.
-		unfold interp_hp_fun, handle_Guarantee, mget, mput in *. rewrite <- ! bind_bind in *.
-		eapply IH; et.
-	- admit. (* need to clarify the relation between fl_src ~ fl_src0 *)
-	- admit. 
-	- steps. unfold interp_hp_fun, handle_Guarantee, mget, mput in *. rewrite <- ! bind_bind in *. et.
-	- steps. unfold interp_hp_fun, handle_Guarantee, mget, mput in *. rewrite <- ! bind_bind in *. et.
-	- steps. force_l. steps. unfold interp_hp_fun, handle_Guarantee, mget, mput in *. rewrite <- ! bind_bind in *. et.
-	- steps. hexploit K; et. i. des.
-		unfold interp_hp_fun, handle_Guarantee, mget, mput in *. rewrite <- ! bind_bind in *.
-		eapply IH; et.
-	- steps. hexploit K; et. i. des.
-		unfold interp_hp_fun, handle_Guarantee, mget, mput in *. rewrite <- ! bind_bind in *.
-		eapply IH; et.
-	- steps. force_r. steps. unfold interp_hp_fun, handle_Guarantee, mget, mput in *. rewrite <- ! bind_bind in *. et.
-	- steps. rewrite ! Any.pair_split. rewrite RUN. s.
-		unfold interp_hp_fun, handle_Guarantee, mget, mput in *. rewrite <- ! bind_bind in *.
-		exploit IHSIM; et.
-	- steps. rewrite ! Any.pair_split. rewrite RUN. s.
-		unfold interp_hp_fun, handle_Guarantee, mget, mput in *. rewrite <- ! bind_bind in *.
-		exploit IHSIM; et.
-	- steps. rewrite interp_hp_Assume. unfold handle_Assume, mget, mput. steps.  
-		unfold interp_hp_fun, handle_Guarantee, mget, mput in *. rewrite <- ! bind_bind in *.
-		hexploit K; et.
-		{ 
-			instantiate (1:= x ⋅ fmr).
-			iIntros "[H H0]". 
-			iPoseProof (_ASSUME0 with "H") as "H".
-			iPoseProof (CUR with "H0") as "H0".
-			iMod "H0". iModIntro. iFrame. 
-		}
-		i. des. eapply IH; et.
-		rewrite <- ! URA.add_assoc.
-		{
-			iIntros "[H H0]".
-			iSplitL "H"; et.
-			iPoseProof (FMR0 with "H0") as "H".
-			rewrite URA.add_assoc. et.
-		}
-	-	steps. rewrite interp_hp_Assume. 
-		hexploit CUR. i.
-		apply iProp_sepconj in H. 2: { admit. }
-		des. rename rq into fmr0.
-		unfold handle_Assume, mget, mput, assume. steps.
-		force_r.
-		instantiate (1:= rp).
-		steps. force_r.
-		{ 
-			clear -H FMR0.
-			assert (URA.wf (fmr ⋅ fr_tgt ⋅ mr_tgt)). { admit. }
-			assert (URA.wf (fmr ⋅ fr_tgt ⋅ mr_tgt ⋅ ε)). { admit. }
-			eapply own_ctx with (ctx := (fr_tgt ⋅ mr_tgt)) in H.
-			uipropall.
-			eapply H in H0. 2: { admit. }
-			des.
-			eapply URA.wf_extends in H0. admit.
-			specialize (H2 ε H1).
-			admit.
-		}
+  - unfold interp_hp_fun, handle_Guarantee, mget, mput, guarantee.
+    hexploit INV. i.
+    eapply iProp_sepconj in H; et. 
+    (* 2: { admit. } *)
+    des.
+    rename rq into fr. rename rp into mr.
+    steps.
+    unfold handle_Guarantee, mget, mput. steps_safe.
+    force_l.
+    instantiate (1:= (c0, ε, fr ⋅ c1 ⋅ mr ⋅ c)).
+    steps_safe.
+    unfold guarantee. force_l.
+    { admit. }
+      (* iIntros "H". iPoseProof (FMR with "H") as "H". iMod "H".
+      rewrite <- URA.add_assoc.
+      iDestruct "H" as "[H H0]". 
+      iPoseProof (H with "H") as "H".
+      replace (c0 ⋅ (fr ⋅ c1) ⋅ (mr ⋅ c)) with (mr ⋅ fr ⋅ (c0 ⋅ c1 ⋅ c)). 2: { r_solve. }
+      iPoseProof (_GUARANTEE with "H0") as "H0".
+      iSplitL "H"; et. *)
+    steps_safe. force_l.
+    { et. }
+    steps_safe. eapply safe_sim_sim; econs; esplits; i.
+    { 
+      econs. esplits; et.
+      { instantiate (1:= ctx). admit. }
+      { admit. }
+      (* { iIntros "H". iPoseProof (H0 with "H") as "H". et. } *)
+    }
+    inv WF0. des.
+    unfold interp_hp_fun, handle_Guarantee, mget, mput, guarantee in K.
+    steps.
+    hexploit K; swap 1 2. 
+    { 
+      instantiate (1:= st_tgt). instantiate (1:= st_src).
+      iIntros "[H1 H2]".
+      iPoseProof (H1 with "H1") as "H1". 
+      iPoseProof (MR with "H2") as "H2".
+      iSplitL "H2"; et.
+    }
+    { admit. }
+    i. des.
+    unfold interp_hp_fun, handle_Guarantee, mget, mput in *. rewrite <- ! bind_bind in *.
+    eapply IH; et.
+    {
+      
+    }
+  - steps. hexploit K; et. i. des.
+    unfold interp_hp_fun, handle_Guarantee, mget, mput in *. rewrite <- ! bind_bind in *.
+    eapply IH; et.
+  - admit. (* need to clarify the relation between fl_src ~ fl_src0 *)
+  - admit. 
+  - steps. unfold interp_hp_fun, handle_Guarantee, mget, mput in *. rewrite <- ! bind_bind in *. et.
+  - steps. unfold interp_hp_fun, handle_Guarantee, mget, mput in *. rewrite <- ! bind_bind in *. et.
+  - steps. force_l. steps. unfold interp_hp_fun, handle_Guarantee, mget, mput in *. rewrite <- ! bind_bind in *. et.
+  - steps. hexploit K; et. i. des.
+    unfold interp_hp_fun, handle_Guarantee, mget, mput in *. rewrite <- ! bind_bind in *.
+    eapply IH; et.
+  - steps. hexploit K; et. i. des.
+    unfold interp_hp_fun, handle_Guarantee, mget, mput in *. rewrite <- ! bind_bind in *.
+    eapply IH; et.
+  - steps. force_r. steps. unfold interp_hp_fun, handle_Guarantee, mget, mput in *. rewrite <- ! bind_bind in *. et.
+  - steps. rewrite ! Any.pair_split. rewrite RUN. s.
+    unfold interp_hp_fun, handle_Guarantee, mget, mput in *. rewrite <- ! bind_bind in *.
+    exploit IHSIM; et.
+  - steps. rewrite ! Any.pair_split. rewrite RUN. s.
+    unfold interp_hp_fun, handle_Guarantee, mget, mput in *. rewrite <- ! bind_bind in *.
+    exploit IHSIM; et.
+  - steps. rewrite interp_hp_Assume. unfold handle_Assume, mget, mput. steps.  
+    unfold interp_hp_fun, handle_Guarantee, mget, mput in *. rewrite <- ! bind_bind in *.
+    hexploit K; et.
+    { 
+      instantiate (1:= x ⋅ fmr).
+      iIntros "[H H0]". 
+      iPoseProof (_ASSUME0 with "H") as "H".
+      iPoseProof (CUR with "H0") as "H0".
+      iMod "H0". iModIntro. iFrame. 
+    }
+    i. des. eapply IH; et.
+    rewrite <- ! URA.add_assoc.
+    {
+      iIntros "[H H0]".
+      iSplitL "H"; et.
+      iPoseProof (FMR0 with "H0") as "H".
+      rewrite URA.add_assoc. et.
+    }
+  -	steps. rewrite interp_hp_Assume. 
+    hexploit CUR. i.
+    apply iProp_sepconj in H. 2: { admit. }
+    des. rename rq into fmr0.
+    unfold handle_Assume, mget, mput, assume. steps.
+    force_r.
+    instantiate (1:= rp).
+    steps. force_r.
+    { 
+      clear -H FMR0.
+      assert (URA.wf (fmr ⋅ fr_tgt ⋅ mr_tgt)). { admit. }
+      assert (URA.wf (fmr ⋅ fr_tgt ⋅ mr_tgt ⋅ ε)). { admit. }
+      eapply own_ctx with (ctx := (fr_tgt ⋅ mr_tgt)) in H.
+      uipropall.
+      eapply H in H0. 2: { admit. }
+      des.
+      eapply URA.wf_extends in H0. admit.
+      specialize (H2 ε H1).
+      admit.
+    }
 
-		steps. force_r; et. 
-		steps.
-		unfold interp_hp_fun, handle_Guarantee, mget, mput in *. rewrite <- ! bind_bind in *.
-		hexploit K; et. 
-		{
-			iIntros "H". iPoseProof (H1 with "H") as "H". et.
-		}
-		i. des. 
-		eapply IH; et.
-		{
-			iIntros "H". 
-			iPoseProof (FMR0 with "H") as "H". iMod "H". rewrite <- ! URA.add_assoc.
-			iDestruct "H" as "[H H0]".
-			replace (fmr0 ⋅ (rp ⋅ (fr_tgt ⋅ mr_tgt))) with ((rp ⋅ fmr0) ⋅ (fr_tgt ⋅ mr_tgt)). 2: { r_solve. }
-			iPoseProof (H with "H") as "H". iMod "H".
-			iSplitL "H"; et.
-		} 
-	- steps. rewrite interp_hp_Guarantee.
-		unfold handle_Guarantee, mget, mput, guarantee. steps.
-		hexploit CUR. i.
-		apply iProp_sepconj in H.  2: { admit. }
-		des. rename rq into fmr0.
-		force_l.
-		instantiate (1:= (rp, fr_tgt, fmr0 ⋅ mr_tgt)).
-		steps. force_l.
-		{
-			iIntros "H". 
-			iPoseProof (FMR0 with "H") as "H". iMod "H".
-			rewrite <- URA.add_assoc.
-			iDestruct "H" as "[H H0]". 
-			iPoseProof (H with "H") as "H". iMod "H".
-			replace (rp ⋅ fr_tgt ⋅ (fmr0 ⋅ mr_tgt)) with (rp ⋅ fmr0 ⋅ (fr_tgt ⋅ mr_tgt)). 2: { r_solve. }
-			iSplitL "H"; et.
-		}
-		steps. force_l; et.
-		steps.
-		hexploit K; et.
-		{
-			iIntros "H". iPoseProof (H1 with "H") as "H". et.	
-		}
-		i. des.
-		unfold interp_hp_fun, handle_Guarantee, mget, mput in *. rewrite <- ! bind_bind in *.
-		eapply IH; et.
-		{
-			replace (fr_tgt ⋅ (fmr0 ⋅ mr_tgt)) with (fmr0 ⋅ fr_tgt ⋅ mr_tgt); r_solve.
-			et.
-		}
-	- steps. rewrite interp_hp_Guarantee. unfold handle_Guarantee, mget, mput, guarantee. steps. 
-		unfold interp_hp_fun, handle_Guarantee, mget, mput in *. rewrite <- ! bind_bind in *.			
-		hexploit K; et.
-		{ 
-			instantiate (1:= (c0 ⋅ fmr)).
-			iIntros "[H H0]".
-			iPoseProof (x0 with "H") as "H".
-			iPoseProof (CUR with "H0") as "H0".
-			iSplitL "H"; et. 	
-		} 
-		i. des.
-		eapply IH; et.
-		{
-			iIntros "H".
-			iPoseProof (FMR0 with "H") as "H". iMod "H".
-			rewrite <- URA.add_assoc. 
-			iDestruct "H" as "[H H0]".
-			iPoseProof (x with "H0") as "H0". iMod "H0".
-			replace (c0 ⋅ fmr ⋅ c1 ⋅ c) with (fmr ⋅ (c0 ⋅ c1 ⋅ c)). 2: { r_solve. }
-			iSplitL "H"; et.
-		}
-	- gstep. econs. gfinal. left. eapply CIH; et. 
-	
-		(* (fr_src ⋅ mr_src) -> fmr in 'SIM' *)
+    steps. force_r; et. 
+    steps.
+    unfold interp_hp_fun, handle_Guarantee, mget, mput in *. rewrite <- ! bind_bind in *.
+    hexploit K; et. 
+    {
+      iIntros "H". iPoseProof (H1 with "H") as "H". et.
+    }
+    i. des. 
+    eapply IH; et.
+    {
+      iIntros "H". 
+      iPoseProof (FMR0 with "H") as "H". iMod "H". rewrite <- ! URA.add_assoc.
+      iDestruct "H" as "[H H0]".
+      replace (fmr0 ⋅ (rp ⋅ (fr_tgt ⋅ mr_tgt))) with ((rp ⋅ fmr0) ⋅ (fr_tgt ⋅ mr_tgt)). 2: { r_solve. }
+      iPoseProof (H with "H") as "H". iMod "H".
+      iSplitL "H"; et.
+    } 
+  - steps. rewrite interp_hp_Guarantee.
+    unfold handle_Guarantee, mget, mput, guarantee. steps.
+    hexploit CUR. i.
+    apply iProp_sepconj in H.  2: { admit. }
+    des. rename rq into fmr0.
+    force_l.
+    instantiate (1:= (rp, fr_tgt, fmr0 ⋅ mr_tgt)).
+    steps. force_l.
+    {
+      iIntros "H". 
+      iPoseProof (FMR0 with "H") as "H". iMod "H".
+      rewrite <- URA.add_assoc.
+      iDestruct "H" as "[H H0]". 
+      iPoseProof (H with "H") as "H". iMod "H".
+      replace (rp ⋅ fr_tgt ⋅ (fmr0 ⋅ mr_tgt)) with (rp ⋅ fmr0 ⋅ (fr_tgt ⋅ mr_tgt)). 2: { r_solve. }
+      iSplitL "H"; et.
+    }
+    steps. force_l; et.
+    steps.
+    hexploit K; et.
+    {
+      iIntros "H". iPoseProof (H1 with "H") as "H". et.	
+    }
+    i. des.
+    unfold interp_hp_fun, handle_Guarantee, mget, mput in *. rewrite <- ! bind_bind in *.
+    eapply IH; et.
+    {
+      replace (fr_tgt ⋅ (fmr0 ⋅ mr_tgt)) with (fmr0 ⋅ fr_tgt ⋅ mr_tgt); r_solve.
+      et.
+    }
+  - steps. rewrite interp_hp_Guarantee. unfold handle_Guarantee, mget, mput, guarantee. steps. 
+    unfold interp_hp_fun, handle_Guarantee, mget, mput in *. rewrite <- ! bind_bind in *.			
+    hexploit K; et.
+    { 
+      instantiate (1:= (c0 ⋅ fmr)).
+      iIntros "[H H0]".
+      iPoseProof (x0 with "H") as "H".
+      iPoseProof (CUR with "H0") as "H0".
+      iSplitL "H"; et. 	
+    } 
+    i. des.
+    eapply IH; et.
+    {
+      iIntros "H".
+      iPoseProof (FMR0 with "H") as "H". iMod "H".
+      rewrite <- URA.add_assoc. 
+      iDestruct "H" as "[H H0]".
+      iPoseProof (x with "H0") as "H0". iMod "H0".
+      replace (c0 ⋅ fmr ⋅ c1 ⋅ c) with (fmr ⋅ (c0 ⋅ c1 ⋅ c)). 2: { r_solve. }
+      iSplitL "H"; et.
+    }
+  - gstep. econs. gfinal. left. eapply CIH; et. 
+  
+    (* (fr_src ⋅ mr_src) -> fmr in 'SIM' *)
 Admitted.
 
 
 
 
 
-	Inductive hpsim_adeq_rel : Σ -> (itree hAGEs Any.t)-> (itree Es (Σ * Any.t)) -> Σ -> (itree hAGEs Any.t)-> (itree Es (Σ * Any.t)) -> Prop :=
-	| hpsim_adeq_base (fr fr': Σ) st st' 
-		: hpsim_adeq_rel fr (Ret st) (@interp_hp_fun Σ Any.t (Ret st) fr)
-										 fr' (Ret st') (@interp_hp_fun Σ Any.t (Ret st') fr')
+  Inductive hpsim_adeq_rel : Σ -> (itree hAGEs Any.t)-> (itree Es (Σ * Any.t)) -> Σ -> (itree hAGEs Any.t)-> (itree Es (Σ * Any.t)) -> Prop :=
+  | hpsim_adeq_base (fr fr': Σ) st st' 
+    : hpsim_adeq_rel fr (Ret st) (@interp_hp_fun Σ Any.t (Ret st) fr)
+                     fr' (Ret st') (@interp_hp_fun Σ Any.t (Ret st') fr')
 
-	| hpsim_adeq_seq itrH0 itrH1 itrL0 itrL1 itrH0' itrH1' itrL0' itrL1' (fr fr': Σ)
-			(ITR0: itrL0 = @interp_hp_fun Σ Any.t itrH0)
-			(ITR0': itrL0' = @interp_hp_fun Σ Any.t itrH0')
-			(ADEQ: forall st st',
-							hpsim_adeq_rel ε (itrH1 st) (itrL1 st (ε:Σ)) 
-														 ε (itrH1' st') (itrL1' st' (ε:Σ)))
-		: hpsim_adeq_rel fr (st0 <- itrH0;; itrH1 st0) ('(_, st1) <- (itrL0 fr);; (itrL1 st1 ε))
-										 fr' (st0 <- itrH0';; itrH1' st0) ('(_, st1) <- (itrL0' fr');; (itrL1' st1 ε))
-	.
+  | hpsim_adeq_seq itrH0 itrH1 itrL0 itrL1 itrH0' itrH1' itrL0' itrL1' (fr fr': Σ)
+      (ITR0: itrL0 = @interp_hp_fun Σ Any.t itrH0)
+      (ITR0': itrL0' = @interp_hp_fun Σ Any.t itrH0')
+      (ADEQ: forall st st',
+              hpsim_adeq_rel ε (itrH1 st) (itrL1 st (ε:Σ)) 
+                             ε (itrH1' st') (itrL1' st' (ε:Σ)))
+    : hpsim_adeq_rel fr (st0 <- itrH0;; itrH1 st0) ('(_, st1) <- (itrL0 fr);; (itrL1 st1 ε))
+                     fr' (st0 <- itrH0';; itrH1' st0) ('(_, st1) <- (itrL0' fr');; (itrL1' st1 ε))
+  .
 
 
   Lemma hpsim_adequacy
-			(fl_src0 fl_tgt0: alist string (Any.t -> itree Es Any.t)) 
-			(FLS: fl_src0 = List.map (fun '(s, f) => (s, interp_hp_fun f)) fl_src)
-			(FLT: fl_tgt0 = List.map (fun '(s, f) => (s, interp_hp_fun f)) fl_tgt)
-			p_src p_tgt st_src st_tgt itrH_src itrH_tgt itrL_src itrL_tgt
-			(ctx mr_src mr_tgt fr_src fr_tgt fmr: Σ)
+      (fl_src0 fl_tgt0: alist string (Any.t -> itree Es Any.t)) 
+      (FLS: fl_src0 = List.map (fun '(s, f) => (s, interp_hp_fun f)) fl_src)
+      (FLT: fl_tgt0 = List.map (fun '(s, f) => (s, interp_hp_fun f)) fl_tgt)
+      p_src p_tgt st_src st_tgt itrH_src itrH_tgt itrL_src itrL_tgt
+      (ctx mr_src mr_tgt fr_src fr_tgt fmr: Σ)
       (SIM: hpsim p_src p_tgt (st_src, itrH_src) (st_tgt, itrH_tgt) fmr)
-			(WF: URA.wf (ctx ⋅ fr_src ⋅ mr_src))
-			(FMR: Own (fr_src ⋅ mr_src) ⊢ #=> Own (fmr ⋅ fr_tgt ⋅ mr_tgt))
-			(REL: hpsim_adeq_rel fr_src itrH_src itrL_src fr_tgt itrH_tgt itrL_tgt)
-		:
+      (WF: URA.wf (ctx ⋅ fr_src ⋅ mr_src))
+      (FMR: Own (fr_src ⋅ mr_src) ⊢ #=> Own (fmr ⋅ fr_tgt ⋅ mr_tgt))
+      (REL: hpsim_adeq_rel fr_src itrH_src itrL_src fr_tgt itrH_tgt itrL_tgt)
+    :
 
-			@sim_itree Σ (mk_inv I) eq fl_src0 fl_tgt0 p_src p_tgt ctx 
-			(Any.pair st_src mr_src↑, itrL_src >>= (fun r => Ret (snd r)))
-			(Any.pair st_tgt mr_tgt↑, itrL_tgt >>= (fun r => Ret (snd r))).
+      @sim_itree Σ (mk_inv I) eq fl_src0 fl_tgt0 p_src p_tgt ctx 
+      (Any.pair st_src mr_src↑, itrL_src >>= (fun r => Ret (snd r)))
+      (Any.pair st_tgt mr_tgt↑, itrL_tgt >>= (fun r => Ret (snd r))).
   Proof.
-		revert_until FLT.
-		ginit. gcofix CIH. i.
-		move REL before CIH. revert_until REL. induction REL.
-		{ i. punfold SIM. inv SIM; (try rewrite ! bind_trigger in H3); (try rewrite ! bind_trigger in H5); clarify.
-			-	unfold interp_hp_fun, handle_Guarantee, mput, mget, guarantee. 
-				steps. force_l. instantiate (1:= (c0 ⋅ c1, ε, fmr ⋅ c)).
-				steps. force_l.
-				{  
-					rewrite FMR. 
-					iIntros "H". iMod "H".
-					rewrite <- URA.add_assoc. 
-					iDestruct "H" as "[H H0]".
-					iPoseProof (x with "H0") as "H0". iMod "H0". 
-					iModIntro. r_solve.
-					replace (c0 ⋅ c1 ⋅ fmr ⋅ c) with (c0 ⋅ c1 ⋅ c ⋅ fmr); r_solve.
-					iSplitR "H"; et.
-				}
-				steps. force_l; et.
-				steps.
-				econs; esplits; et. econs; esplits; et.
-				{  
-					eapply own_ctx in FMR. rewrite URA.add_assoc in FMR. eapply own_wf in FMR; et.
-					rewrite <- URA.add_assoc in FMR. rewrite URA.add_assoc in FMR.
-					eapply own_ctx, own_wf in x; et.
-					replace (ctx ⋅ fmr ⋅ (c0 ⋅ c1 ⋅ c)) with (ctx ⋅ fmr ⋅ c ⋅ (c0 ⋅ c1)) in x; r_solve.
-					eapply URA.wf_mon; et.
-				}
-			- pclearbot. punfold SIM0. inv SIM0; (try rewrite ! bind_trigger in H3); (try rewrite ! bind_trigger in H5); clarify.
-				unfold interp_hp_fun, handle_Guarantee, mput, mget, guarantee. steps.
-				force_l. instantiate (1:= (c0 ⋅ c1, ε, fmr ⋅ c)).
-				steps. force_l.
-				{  
-					rewrite FMR. 
-					iIntros "H". iMod "H".
-					rewrite <- URA.add_assoc. 
-					iDestruct "H" as "[H H0]".
-					iPoseProof (x with "H0") as "H0". iMod "H0". 
-					iModIntro. r_solve.
-					replace (c0 ⋅ c1 ⋅ fmr ⋅ c) with (c0 ⋅ c1 ⋅ c ⋅ fmr); r_solve.
-					iSplitR "H"; et.
-				}
-				steps. force_l; et.
-				steps.
-				econs; esplits; et. econs; esplits; et.
-				{  
-					eapply own_ctx in FMR. rewrite URA.add_assoc in FMR. eapply own_wf in FMR; et.
-					rewrite <- URA.add_assoc in FMR. rewrite URA.add_assoc in FMR.
-					eapply own_ctx, own_wf in x; et.
-					replace (ctx ⋅ fmr ⋅ (c0 ⋅ c1 ⋅ c)) with (ctx ⋅ fmr ⋅ c ⋅ (c0 ⋅ c1)) in x; r_solve.
-					eapply URA.wf_mon; et.
-				}
-		}
+    revert_until FLT.
+    ginit. gcofix CIH. i.
+    move REL before CIH. revert_until REL. induction REL.
+    { i. punfold SIM. inv SIM; (try rewrite ! bind_trigger in H3); (try rewrite ! bind_trigger in H5); clarify.
+      -	unfold interp_hp_fun, handle_Guarantee, mput, mget, guarantee. 
+        steps. force_l. instantiate (1:= (c0 ⋅ c1, ε, fmr ⋅ c)).
+        steps. force_l.
+        {  
+          rewrite FMR. 
+          iIntros "H". iMod "H".
+          rewrite <- URA.add_assoc. 
+          iDestruct "H" as "[H H0]".
+          iPoseProof (x with "H0") as "H0". iMod "H0". 
+          iModIntro. r_solve.
+          replace (c0 ⋅ c1 ⋅ fmr ⋅ c) with (c0 ⋅ c1 ⋅ c ⋅ fmr); r_solve.
+          iSplitR "H"; et.
+        }
+        steps. force_l; et.
+        steps.
+        econs; esplits; et. econs; esplits; et.
+        {  
+          eapply own_ctx in FMR. rewrite URA.add_assoc in FMR. eapply own_wf in FMR; et.
+          rewrite <- URA.add_assoc in FMR. rewrite URA.add_assoc in FMR.
+          eapply own_ctx, own_wf in x; et.
+          replace (ctx ⋅ fmr ⋅ (c0 ⋅ c1 ⋅ c)) with (ctx ⋅ fmr ⋅ c ⋅ (c0 ⋅ c1)) in x; r_solve.
+          eapply URA.wf_mon; et.
+        }
+      - pclearbot. punfold SIM0. inv SIM0; (try rewrite ! bind_trigger in H3); (try rewrite ! bind_trigger in H5); clarify.
+        unfold interp_hp_fun, handle_Guarantee, mput, mget, guarantee. steps.
+        force_l. instantiate (1:= (c0 ⋅ c1, ε, fmr ⋅ c)).
+        steps. force_l.
+        {  
+          rewrite FMR. 
+          iIntros "H". iMod "H".
+          rewrite <- URA.add_assoc. 
+          iDestruct "H" as "[H H0]".
+          iPoseProof (x with "H0") as "H0". iMod "H0". 
+          iModIntro. r_solve.
+          replace (c0 ⋅ c1 ⋅ fmr ⋅ c) with (c0 ⋅ c1 ⋅ c ⋅ fmr); r_solve.
+          iSplitR "H"; et.
+        }
+        steps. force_l; et.
+        steps.
+        econs; esplits; et. econs; esplits; et.
+        {  
+          eapply own_ctx in FMR. rewrite URA.add_assoc in FMR. eapply own_wf in FMR; et.
+          rewrite <- URA.add_assoc in FMR. rewrite URA.add_assoc in FMR.
+          eapply own_ctx, own_wf in x; et.
+          replace (ctx ⋅ fmr ⋅ (c0 ⋅ c1 ⋅ c)) with (ctx ⋅ fmr ⋅ c ⋅ (c0 ⋅ c1)) in x; r_solve.
+          eapply URA.wf_mon; et.
+        }
+    }
 
-		i.
-		remember (st_src, ` st0 : Any.t <- itrH0;; itrH1 st0) as sti_src.
-		remember (st_tgt, ` st0 : Any.t <- itrH0';; itrH1' st0) as sti_tgt.
-		move SIM before CIH. revert_until SIM.
-		induction SIM using hpsim_ind; i. 
-		(* ; clarify; unfold interp_hp_fun, handle_Guarantee, mget, mput. *)
-		- 
-			steps.
-			ides itrH0; ides itrH0'; revert H1 H2; try rewrite bind_vis; grind.
-			unfold interp_hp_fun, handle_Guarantee, mget, mput, guarantee.
-			steps. force_l.
-			instantiate (1 := (c0 ⋅ c1, ε, fmr ⋅ c)).
-			steps. force_l.
-			{
-				admit.
-			}
-			steps. force_l; et. steps.
-			specialize (ADEQ r0 r1). depdes ADEQ; cycle 1.
-			{
-				eapply H.
-				{ rewrite <- H1. rewrite <- H2. et. }
-				admit. admit.
-			}
-			
-			rewrite <- x1. rewrite <- x.
-			unfold interp_hp_fun, handle_Guarantee, mget, mput, guarantee.
-			steps. force_l.
-			instantiate (1 := (c3 ⋅ c4, ε, fmr ⋅ c2 )).
-			steps. force_l.
-			{
-				admit.
-			} 
-			steps. force_l; et.
-			steps.
-			econs. esplits; et.
-			{
-				econs. esplits; et.	admit.
-			}
-			rewrite <- H1 in x2.
-			rewrite <- H2 in x0.
-			clarify.
-			
-		- steps. move K at bottom.
-			ides itrH0; ides itrH0'; clarify.
-
-
+    i.
+    remember (st_src, ` st0 : Any.t <- itrH0;; itrH1 st0) as sti_src.
+    remember (st_tgt, ` st0 : Any.t <- itrH0';; itrH1' st0) as sti_tgt.
+    move SIM before CIH. revert_until SIM.
+    induction SIM using hpsim_ind; i. 
+    (* ; clarify; unfold interp_hp_fun, handle_Guarantee, mget, mput. *)
+    - 
+      steps.
+      ides itrH0; ides itrH0'; revert H1 H2; try rewrite bind_vis; grind.
+      unfold interp_hp_fun, handle_Guarantee, mget, mput, guarantee.
+      steps. force_l.
+      instantiate (1 := (c0 ⋅ c1, ε, fmr ⋅ c)).
+      steps. force_l.
+      {
+        admit.
+      }
+      steps. force_l; et. steps.
+      specialize (ADEQ r0 r1). depdes ADEQ; cycle 1.
+      {
+        eapply H.
+        { rewrite <- H1. rewrite <- H2. et. }
+        admit. admit.
+      }
+      
+      rewrite <- x1. rewrite <- x.
+      unfold interp_hp_fun, handle_Guarantee, mget, mput, guarantee.
+      steps. force_l.
+      instantiate (1 := (c3 ⋅ c4, ε, fmr ⋅ c2 )).
+      steps. force_l.
+      {
+        admit.
+      } 
+      steps. force_l; et.
+      steps.
+      econs. esplits; et.
+      {
+        econs. esplits; et.	admit.
+      }
+      rewrite <- H1 in x2.
+      rewrite <- H2 in x0.
+      clarify.
+      
+    - steps. move K at bottom.
+      ides itrH0; ides itrH0'; clarify.
 
 
-			{
-					
-			}
-				admit. steps. 
-				force_l. steps. admit. steps. eapply H; et.
 
 
-		unfold interp_hp_fun, handle_Guarantee, mget, mput.
-			steps.
+      {
+          
+      }
+        admit. steps. 
+        force_l. steps. admit. steps. eapply H; et.
 
-			force_l. instantiate (1 := (c0 ⋅ c1, ε, fmr ⋅ c)). steps.
-			unfold guarantee. force_l.
-			{ 
-				rewrite FMR. 
-				iIntros "H". iMod "H".
-				rewrite <- URA.add_assoc. 
-				iDestruct "H" as "[H1 H2]".
-				iPoseProof (_GUARANTEE with "H2") as "H2".
-				iMod "H2".
-				iModIntro. r_solve.
-				iDestruct "H2" as "[H3 H4]".
-				iSplitR "H4"; et.
-				iCombine "H3 H1" as "H". et.
-			} 
-			steps. force_l. 
-			{ iIntros "H". et. } 
-			steps. econs; esplits; et.
-			+ econs. esplits; et.
-				eapply own_ctx with (ctx:= ctx ⋅ fmr) in _GUARANTEE.
-				eapply own_ctx with (ctx:= ctx) in FMR.
-				rewrite <- URA.add_assoc in WF. eapply own_wf in FMR; et.
-				rewrite ! URA.add_assoc in FMR.
-				rewrite URA.add_assoc in _GUARANTEE.
-				eapply own_wf in _GUARANTEE; et.
-				replace (ctx ⋅ fmr ⋅ (c0 ⋅ c1 ⋅ c)) with (ctx ⋅ (fmr ⋅ c) ⋅ c0 ⋅ c1) in _GUARANTEE. 2: { r_solve. }
-				do 2 eapply URA.wf_mon; et.
-		- hexploit INV. i.
-			eapply iProp_sepconj in H. et.
-			des.
-			rename rq into fr. rename rp into mr.
-			steps.
-			unfold handle_Guarantee, mget, mput. steps_safe.
-			force_l.
-			instantiate (1:= (c0, fr ⋅ c1, mr ⋅ c)).
-			rename c1 into fr_tgt'. rename c into mr_tgt'.
-			steps_safe.
-			unfold guarantee. force_l.
-			{ 
-				iIntros "H". iPoseProof (FMR with "H") as "H". iMod "H".
-				rewrite <- URA.add_assoc.
-				iDestruct "H" as "[H H0]". 
-				iPoseProof (H with "H") as "H".
-				replace (c0 ⋅ (fr ⋅ fr_tgt') ⋅ (mr ⋅ mr_tgt')) with (mr ⋅ fr ⋅ (c0 ⋅ fr_tgt' ⋅ mr_tgt')). 2: { r_solve. }
-				iPoseProof (_GUARANTEE with "H0") as "H0".
-				iSplitL "H"; et.
-			}
-			steps_safe. force_l.
-			{ et. }
-			steps_safe. eapply safe_sim_sim; econs; i.
-			exists (fr ⋅ ctx). esplits.
-			{ 
-				econs. esplits; et.
-				{
-					eapply own_ctx with (ctx:= ctx ⋅ fmr) in _GUARANTEE.
-					eapply own_ctx with (ctx:= ctx) in FMR.
-					rewrite <- URA.add_assoc in WF. eapply own_wf in FMR; et.
-					rewrite ! URA.add_assoc in FMR.
-					rewrite URA.add_assoc in _GUARANTEE.
-					eapply own_wf in _GUARANTEE; et.
-					rewrite URA.add_comm in _GUARANTEE. rewrite URA.add_assoc in _GUARANTEE.
-					eapply own_ctx in H. eapply own_wf in H; et.
-					replace (c0 ⋅ fr_tgt' ⋅ mr_tgt' ⋅ ctx ⋅ (mr ⋅ fr)) with (fr ⋅ ctx ⋅ mr ⋅ mr_tgt' ⋅ (c0 ⋅ fr_tgt')) in H; r_solve.
-					eapply URA.wf_mon; et.
-				} 
-				iIntros "H". iPoseProof (H0 with "H") as "H". et.
-			}
-			i. inv WF0. des.
-			unfold interp_hp_fun, handle_Guarantee, mget, mput, guarantee in K.
-			hexploit K; swap 1 2.
-			{ 
-				iIntros "[H1 H2]".
-				iPoseProof (H1 with "H1") as "H1". 
-				iPoseProof (MR with "H2") as "H2".
-				iSplitL "H2"; et.
-			}
-			{
-				eapply own_ctx in MRS. eapply own_wf in MRS; et.
-				replace (fr ⋅ ctx ⋅ (mr0 ⋅ mr_tgt0)) with (fr ⋅ mr0 ⋅ (ctx ⋅ mr_tgt0)) in MRS; r_solve.
-				eapply URA.wf_mon; et.				
-			}
-			i. des.
-			steps. 
-			unfold interp_hp_fun, handle_Guarantee, mget, mput in *. rewrite <- ! bind_bind in *.
-			eapply IH; et.
-			{ 
-				iIntros "[H H0]".
-				iPoseProof (MRS with "H0") as "H0".
-				replace (fr ⋅ mr0 ⋅ fr_tgt' ⋅ mr_tgt0) with (fr ⋅ fr_tgt' ⋅ (mr0 ⋅ mr_tgt0)). 2: { r_solve. }  
-				iSplitL "H"; et.
-			}
-			{
-				clear IH.
 
-				admit.	
-			}
-		- steps. hexploit K; et. i. des.
-			unfold interp_hp_fun, handle_Guarantee, mget, mput in *. rewrite <- ! bind_bind in *.
-			eapply IH; et.
-		- steps. unfold handle_Guarantee, mget, mput, guarantee. steps.
-			force_l.
-			instantiate (1:= (ε, ε, fr_src ⋅ mr_src)).
-			steps. force_l. { r_solve. et. }
-			steps. force_l; et. 
-			steps. 
-			{ 
-				instantiate (1:= interp_hp_fun f).
-				rewrite alist_find_map. rewrite FUN. et.
-			}
-			unfold interp_hp_fun, interp_hp_fun. steps.
-			do 3 rewrite <- bind_bind in *.
-			(* set (` x : Σ * Any.t <- interp_hp (f varg) ε;; (let '(_, x0) := x in Ret x0)) as itr. *)
-			(* assert () *)
-			set ((` x : Σ * Any.t <- (` x : Any.t <- (` x : Σ * Any.t <- interp_hp (f varg) ε;; (let '(_, x0) := x in Ret x0));; (tau;; Ret (fr_src, x)));;
-			interp_hp (k_src x.2) x.1)) as itr0.
-			set (interp_hp (` x : Any.t <- (f varg);; k_src x) fr_src) as itr1.
-			assert (itr0 = itr1 ). {
-				unfold itr0, itr1. grind. rewrite interp_hp_bind.	
-			admit. }
-			rewrite H. unfold itr1.
-			(* assert (itr_src = interp_hp (` x : Any.t <- (f varg);; ` x : Σ * Any.t <- (k_src x)) fr_src).
-			{ unfold itr_src. grind. }
-			rewrite <- interp_hp_bind. *)
-			unfold interp_hp_fun, handle_Guarantee, mget, mput in *. rewrite <- ! bind_bind in *.
-			eapply IHSIM; et.
-	
-		- admit. 
-		- steps. unfold interp_hp_fun, handle_Guarantee, mget, mput in *. rewrite <- ! bind_bind in *. et.
-		- steps. unfold interp_hp_fun, handle_Guarantee, mget, mput in *. rewrite <- ! bind_bind in *. et.
-		- steps. force_l. steps. unfold interp_hp_fun, handle_Guarantee, mget, mput in *. rewrite <- ! bind_bind in *. et.
-		- steps. hexploit K; et. i. des.
-			unfold interp_hp_fun, handle_Guarantee, mget, mput in *. rewrite <- ! bind_bind in *.
-			eapply IH; et.
-		- steps. hexploit K; et. i. des.
-			unfold interp_hp_fun, handle_Guarantee, mget, mput in *. rewrite <- ! bind_bind in *.
-			eapply IH; et.
-		- steps. force_r. steps. unfold interp_hp_fun, handle_Guarantee, mget, mput in *. rewrite <- ! bind_bind in *. et.
-		- steps. rewrite ! Any.pair_split. rewrite RUN. s.
-			unfold interp_hp_fun, handle_Guarantee, mget, mput in *. rewrite <- ! bind_bind in *.
-			eapply IHSIM; et.
-		- steps. rewrite ! Any.pair_split. rewrite RUN. s.
-			unfold interp_hp_fun, handle_Guarantee, mget, mput in *. rewrite <- ! bind_bind in *.
-			eapply IHSIM; et.
-		- steps. rewrite interp_hp_Assume. unfold handle_Assume, mget, mput. steps.  
-			unfold interp_hp_fun, handle_Guarantee, mget, mput in *. rewrite <- ! bind_bind in *.
-			(* hexploit K. *)
-			hexploit (K (x ⋅ fmr)). et.
-			{ 
-				eapply own_ctx in FMR0. eapply own_wf in FMR0; cycle 1.
-				{ rewrite URA.add_assoc; et.  }
-				{ rewrite ! URA.add_assoc in FMR0. do 2 eapply URA.wf_mon; et.  }
-			}
-			et.
-			{
-				iIntros "[H H0]". 
-				iPoseProof (_ASSUME0 with "H") as "H".
-				iPoseProof (CUR with "H0") as "H0".
-				iMod "H0". iModIntro. iFrame. 
-			}
-			i. des. eapply IH; et.
-			{
-				rewrite <- ! URA.add_assoc.
-				iIntros "[H H0]".
-				iSplitL "H"; et.
-				iPoseProof (FMR0 with "H0") as "H".
-				rewrite URA.add_assoc. et.
-			}
-			{
-				clear IH. admit.
-			}
-		-	steps. rewrite interp_hp_Assume. 
-			hexploit CUR. i.
-			apply iProp_sepconj in H.
-			des. rename rq into fmr0.
-			unfold handle_Assume, mget, mput, assume. steps.
-			force_r.
-			instantiate (1:= rp).
-			steps. force_r.
-			{ 
-				eapply own_ctx in FMR0. rewrite URA.add_assoc in FMR0. eapply own_wf in FMR0; et.
-				replace (ctx ⋅ (fmr ⋅ fr_tgt ⋅ mr_tgt)) with (ctx ⋅ fr_tgt ⋅ mr_tgt ⋅ fmr) in FMR0; r_solve.
-				eapply own_ctx in H. eapply own_wf in H; et.
-				replace (ctx ⋅ fr_tgt ⋅ mr_tgt ⋅ (rp ⋅ fmr0)) with (rp ⋅ fr_tgt ⋅ mr_tgt ⋅ (ctx ⋅ fmr0)) in H; r_solve.
-				eapply URA.wf_mon; et.	
-			}
-			steps. force_r; et. 
-			steps.
-			unfold interp_hp_fun, handle_Guarantee, mget, mput in *. rewrite <- ! bind_bind in *.
-			hexploit (K fmr0).
-			{
-				eapply own_ctx in FMR0. rewrite URA.add_assoc in FMR0; et. eapply own_wf in FMR0; et.
-				replace (ctx ⋅ (fmr ⋅ fr_tgt ⋅ mr_tgt )) with (fmr ⋅ (ctx ⋅ fr_tgt ⋅ mr_tgt)) in FMR0; r_solve.
-				eapply URA.wf_mon in FMR0. eapply own_wf in H; et.
-				rewrite URA.add_comm in H. eapply URA.wf_mon; et.
-			}
-			{ 
-				iIntros "H". iPoseProof (H1 with "H") as "H". et.
-			}
-			i. des.
-			eapply IH; et.
-			{
-				clear IH.
-				iIntros "H". iPoseProof (FMR0 with "H") as "H".
-				rewrite <- URA.add_assoc. iMod "H". iDestruct "H" as "[H H0]".
-				r_solve. rewrite <- URA.add_assoc. iSplitL "H"; et.
-				iPoseProof (H with "H") as "H". iMod "H".
-				iDestruct "H" as "[H H0]". iSplitL "H0"; et.  				
-			}
-		- steps. rewrite interp_hp_Guarantee.
-			unfold handle_Guarantee, mget, mput, guarantee. steps.
-			hexploit CUR. i.
-			apply iProp_sepconj in H.
-			des. rename rq into fmr0.
-			force_l.
-			instantiate (1:= (rp, fr_tgt, fmr0 ⋅ mr_tgt)).
-			steps. force_l.
-			{
-				iIntros "H". 
-				iPoseProof (FMR0 with "H") as "H". iMod "H".
-				rewrite <- URA.add_assoc.
-				iDestruct "H" as "[H H0]". 
-				iPoseProof (H with "H") as "H". iMod "H".
-				replace (rp ⋅ fr_tgt ⋅ (fmr0 ⋅ mr_tgt)) with (rp ⋅ fmr0 ⋅ (fr_tgt ⋅ mr_tgt)). 2: { r_solve. }
-				iSplitL "H"; et.
-			}
-			steps. force_l; et.
-			steps.
-			hexploit (K fmr0); et.
-			{
-				eapply own_ctx in FMR0. rewrite URA.add_assoc in FMR0. eapply own_wf in FMR0; et.
-				replace (ctx ⋅ (fmr ⋅ fr_tgt ⋅ mr_tgt)) with (ctx ⋅ fr_tgt ⋅ mr_tgt ⋅ fmr) in FMR0; r_solve.
-				eapply own_ctx, own_wf in H; et.
-				rewrite URA.add_assoc in H.
-				eapply URA.wf_mon. rewrite URA.add_comm. et.
-			}
-			{
-				iIntros "H". iPoseProof (H1 with "H") as "H". et.	
-			}
-			i. des.
-			unfold interp_hp_fun, handle_Guarantee, mget, mput in *. rewrite <- ! bind_bind in *.
-			eapply IH; et.
-			{
-				replace (fr_tgt ⋅ (fmr0 ⋅ mr_tgt)) with (fmr0 ⋅ fr_tgt ⋅ mr_tgt); r_solve.
-				et.
-			}
-			{
-				clear IH. 
-				eapply own_ctx in FMR0. rewrite URA.add_assoc in FMR0. eapply own_wf in FMR0; et.
-				replace (ctx ⋅ (fmr ⋅ fr_tgt ⋅ mr_tgt)) with (ctx ⋅ fr_tgt ⋅ mr_tgt ⋅ fmr) in FMR0; r_solve.
-				eapply own_ctx, own_wf in H; et.
-				replace (ctx ⋅ fr_tgt ⋅ mr_tgt ⋅ (rp ⋅ fmr0)) with (ctx ⋅ fr_tgt ⋅ fmr0 ⋅ mr_tgt ⋅ rp) in H; r_solve.
-				eapply URA.wf_mon; et.
-			}
-		- steps. rewrite interp_hp_Guarantee. unfold handle_Guarantee, mget, mput, guarantee. steps. 
-			unfold interp_hp_fun, handle_Guarantee, mget, mput in *. rewrite <- ! bind_bind in *.			
-			hexploit (K (c0 ⋅ fmr)). 
-			{
-				eapply own_ctx in FMR0. rewrite URA.add_assoc in FMR0. eapply own_wf in FMR0; et.
-				rewrite <- URA.add_assoc in FMR0. rewrite URA.add_assoc in FMR0.
-				eapply own_ctx, own_wf in x; et.
-				replace (ctx ⋅ fmr ⋅ (c0 ⋅ c1 ⋅ c)) with (c0 ⋅ fmr ⋅ (ctx ⋅ c1 ⋅ c)) in x; r_solve.
-				eapply URA.wf_mon; et.
-			}
-			{ 
-				iIntros "[H H0]".
-				iPoseProof (x0 with "H") as "H".
-				iPoseProof (CUR with "H0") as "H0".
-				iSplitL "H"; et. 	
-			} 
-			i. des.
-			eapply IH; et.
-			{
-				iIntros "H".
-				iPoseProof (FMR0 with "H") as "H". iMod "H".
-				rewrite <- URA.add_assoc. 
-				iDestruct "H" as "[H H0]".
-				iPoseProof (x with "H0") as "H0". iMod "H0".
-				replace (c0 ⋅ fmr ⋅ c1 ⋅ c) with (fmr ⋅ (c0 ⋅ c1 ⋅ c)). 2: { r_solve. }
-				iSplitL "H"; et.
-			}
-		- gstep. econs. gfinal. left. eapply CIH; et. 
-	Admitted.
+    unfold interp_hp_fun, handle_Guarantee, mget, mput.
+      steps.
+
+      force_l. instantiate (1 := (c0 ⋅ c1, ε, fmr ⋅ c)). steps.
+      unfold guarantee. force_l.
+      { 
+        rewrite FMR. 
+        iIntros "H". iMod "H".
+        rewrite <- URA.add_assoc. 
+        iDestruct "H" as "[H1 H2]".
+        iPoseProof (_GUARANTEE with "H2") as "H2".
+        iMod "H2".
+        iModIntro. r_solve.
+        iDestruct "H2" as "[H3 H4]".
+        iSplitR "H4"; et.
+        iCombine "H3 H1" as "H". et.
+      } 
+      steps. force_l. 
+      { iIntros "H". et. } 
+      steps. econs; esplits; et.
+      + econs. esplits; et.
+        eapply own_ctx with (ctx:= ctx ⋅ fmr) in _GUARANTEE.
+        eapply own_ctx with (ctx:= ctx) in FMR.
+        rewrite <- URA.add_assoc in WF. eapply own_wf in FMR; et.
+        rewrite ! URA.add_assoc in FMR.
+        rewrite URA.add_assoc in _GUARANTEE.
+        eapply own_wf in _GUARANTEE; et.
+        replace (ctx ⋅ fmr ⋅ (c0 ⋅ c1 ⋅ c)) with (ctx ⋅ (fmr ⋅ c) ⋅ c0 ⋅ c1) in _GUARANTEE. 2: { r_solve. }
+        do 2 eapply URA.wf_mon; et.
+    - hexploit INV. i.
+      eapply iProp_sepconj in H. et.
+      des.
+      rename rq into fr. rename rp into mr.
+      steps.
+      unfold handle_Guarantee, mget, mput. steps_safe.
+      force_l.
+      instantiate (1:= (c0, fr ⋅ c1, mr ⋅ c)).
+      rename c1 into fr_tgt'. rename c into mr_tgt'.
+      steps_safe.
+      unfold guarantee. force_l.
+      { 
+        iIntros "H". iPoseProof (FMR with "H") as "H". iMod "H".
+        rewrite <- URA.add_assoc.
+        iDestruct "H" as "[H H0]". 
+        iPoseProof (H with "H") as "H".
+        replace (c0 ⋅ (fr ⋅ fr_tgt') ⋅ (mr ⋅ mr_tgt')) with (mr ⋅ fr ⋅ (c0 ⋅ fr_tgt' ⋅ mr_tgt')). 2: { r_solve. }
+        iPoseProof (_GUARANTEE with "H0") as "H0".
+        iSplitL "H"; et.
+      }
+      steps_safe. force_l.
+      { et. }
+      steps_safe. eapply safe_sim_sim; econs; i.
+      exists (fr ⋅ ctx). esplits.
+      { 
+        econs. esplits; et.
+        {
+          eapply own_ctx with (ctx:= ctx ⋅ fmr) in _GUARANTEE.
+          eapply own_ctx with (ctx:= ctx) in FMR.
+          rewrite <- URA.add_assoc in WF. eapply own_wf in FMR; et.
+          rewrite ! URA.add_assoc in FMR.
+          rewrite URA.add_assoc in _GUARANTEE.
+          eapply own_wf in _GUARANTEE; et.
+          rewrite URA.add_comm in _GUARANTEE. rewrite URA.add_assoc in _GUARANTEE.
+          eapply own_ctx in H. eapply own_wf in H; et.
+          replace (c0 ⋅ fr_tgt' ⋅ mr_tgt' ⋅ ctx ⋅ (mr ⋅ fr)) with (fr ⋅ ctx ⋅ mr ⋅ mr_tgt' ⋅ (c0 ⋅ fr_tgt')) in H; r_solve.
+          eapply URA.wf_mon; et.
+        } 
+        iIntros "H". iPoseProof (H0 with "H") as "H". et.
+      }
+      i. inv WF0. des.
+      unfold interp_hp_fun, handle_Guarantee, mget, mput, guarantee in K.
+      hexploit K; swap 1 2.
+      { 
+        iIntros "[H1 H2]".
+        iPoseProof (H1 with "H1") as "H1". 
+        iPoseProof (MR with "H2") as "H2".
+        iSplitL "H2"; et.
+      }
+      {
+        eapply own_ctx in MRS. eapply own_wf in MRS; et.
+        replace (fr ⋅ ctx ⋅ (mr0 ⋅ mr_tgt0)) with (fr ⋅ mr0 ⋅ (ctx ⋅ mr_tgt0)) in MRS; r_solve.
+        eapply URA.wf_mon; et.				
+      }
+      i. des.
+      steps. 
+      unfold interp_hp_fun, handle_Guarantee, mget, mput in *. rewrite <- ! bind_bind in *.
+      eapply IH; et.
+      { 
+        iIntros "[H H0]".
+        iPoseProof (MRS with "H0") as "H0".
+        replace (fr ⋅ mr0 ⋅ fr_tgt' ⋅ mr_tgt0) with (fr ⋅ fr_tgt' ⋅ (mr0 ⋅ mr_tgt0)). 2: { r_solve. }  
+        iSplitL "H"; et.
+      }
+      {
+        clear IH.
+
+        admit.	
+      }
+    - steps. hexploit K; et. i. des.
+      unfold interp_hp_fun, handle_Guarantee, mget, mput in *. rewrite <- ! bind_bind in *.
+      eapply IH; et.
+    - steps. unfold handle_Guarantee, mget, mput, guarantee. steps.
+      force_l.
+      instantiate (1:= (ε, ε, fr_src ⋅ mr_src)).
+      steps. force_l. { r_solve. et. }
+      steps. force_l; et. 
+      steps. 
+      { 
+        instantiate (1:= interp_hp_fun f).
+        rewrite alist_find_map. rewrite FUN. et.
+      }
+      unfold interp_hp_fun, interp_hp_fun. steps.
+      do 3 rewrite <- bind_bind in *.
+      (* set (` x : Σ * Any.t <- interp_hp (f varg) ε;; (let '(_, x0) := x in Ret x0)) as itr. *)
+      (* assert () *)
+      set ((` x : Σ * Any.t <- (` x : Any.t <- (` x : Σ * Any.t <- interp_hp (f varg) ε;; (let '(_, x0) := x in Ret x0));; (tau;; Ret (fr_src, x)));;
+      interp_hp (k_src x.2) x.1)) as itr0.
+      set (interp_hp (` x : Any.t <- (f varg);; k_src x) fr_src) as itr1.
+      assert (itr0 = itr1 ). {
+        unfold itr0, itr1. grind. rewrite interp_hp_bind.	
+      admit. }
+      rewrite H. unfold itr1.
+      (* assert (itr_src = interp_hp (` x : Any.t <- (f varg);; ` x : Σ * Any.t <- (k_src x)) fr_src).
+      { unfold itr_src. grind. }
+      rewrite <- interp_hp_bind. *)
+      unfold interp_hp_fun, handle_Guarantee, mget, mput in *. rewrite <- ! bind_bind in *.
+      eapply IHSIM; et.
+  
+    - admit. 
+    - steps. unfold interp_hp_fun, handle_Guarantee, mget, mput in *. rewrite <- ! bind_bind in *. et.
+    - steps. unfold interp_hp_fun, handle_Guarantee, mget, mput in *. rewrite <- ! bind_bind in *. et.
+    - steps. force_l. steps. unfold interp_hp_fun, handle_Guarantee, mget, mput in *. rewrite <- ! bind_bind in *. et.
+    - steps. hexploit K; et. i. des.
+      unfold interp_hp_fun, handle_Guarantee, mget, mput in *. rewrite <- ! bind_bind in *.
+      eapply IH; et.
+    - steps. hexploit K; et. i. des.
+      unfold interp_hp_fun, handle_Guarantee, mget, mput in *. rewrite <- ! bind_bind in *.
+      eapply IH; et.
+    - steps. force_r. steps. unfold interp_hp_fun, handle_Guarantee, mget, mput in *. rewrite <- ! bind_bind in *. et.
+    - steps. rewrite ! Any.pair_split. rewrite RUN. s.
+      unfold interp_hp_fun, handle_Guarantee, mget, mput in *. rewrite <- ! bind_bind in *.
+      eapply IHSIM; et.
+    - steps. rewrite ! Any.pair_split. rewrite RUN. s.
+      unfold interp_hp_fun, handle_Guarantee, mget, mput in *. rewrite <- ! bind_bind in *.
+      eapply IHSIM; et.
+    - steps. rewrite interp_hp_Assume. unfold handle_Assume, mget, mput. steps.  
+      unfold interp_hp_fun, handle_Guarantee, mget, mput in *. rewrite <- ! bind_bind in *.
+      (* hexploit K. *)
+      hexploit (K (x ⋅ fmr)). et.
+      { 
+        eapply own_ctx in FMR0. eapply own_wf in FMR0; cycle 1.
+        { rewrite URA.add_assoc; et.  }
+        { rewrite ! URA.add_assoc in FMR0. do 2 eapply URA.wf_mon; et.  }
+      }
+      et.
+      {
+        iIntros "[H H0]". 
+        iPoseProof (_ASSUME0 with "H") as "H".
+        iPoseProof (CUR with "H0") as "H0".
+        iMod "H0". iModIntro. iFrame. 
+      }
+      i. des. eapply IH; et.
+      {
+        rewrite <- ! URA.add_assoc.
+        iIntros "[H H0]".
+        iSplitL "H"; et.
+        iPoseProof (FMR0 with "H0") as "H".
+        rewrite URA.add_assoc. et.
+      }
+      {
+        clear IH. admit.
+      }
+    -	steps. rewrite interp_hp_Assume. 
+      hexploit CUR. i.
+      apply iProp_sepconj in H.
+      des. rename rq into fmr0.
+      unfold handle_Assume, mget, mput, assume. steps.
+      force_r.
+      instantiate (1:= rp).
+      steps. force_r.
+      { 
+        eapply own_ctx in FMR0. rewrite URA.add_assoc in FMR0. eapply own_wf in FMR0; et.
+        replace (ctx ⋅ (fmr ⋅ fr_tgt ⋅ mr_tgt)) with (ctx ⋅ fr_tgt ⋅ mr_tgt ⋅ fmr) in FMR0; r_solve.
+        eapply own_ctx in H. eapply own_wf in H; et.
+        replace (ctx ⋅ fr_tgt ⋅ mr_tgt ⋅ (rp ⋅ fmr0)) with (rp ⋅ fr_tgt ⋅ mr_tgt ⋅ (ctx ⋅ fmr0)) in H; r_solve.
+        eapply URA.wf_mon; et.	
+      }
+      steps. force_r; et. 
+      steps.
+      unfold interp_hp_fun, handle_Guarantee, mget, mput in *. rewrite <- ! bind_bind in *.
+      hexploit (K fmr0).
+      {
+        eapply own_ctx in FMR0. rewrite URA.add_assoc in FMR0; et. eapply own_wf in FMR0; et.
+        replace (ctx ⋅ (fmr ⋅ fr_tgt ⋅ mr_tgt )) with (fmr ⋅ (ctx ⋅ fr_tgt ⋅ mr_tgt)) in FMR0; r_solve.
+        eapply URA.wf_mon in FMR0. eapply own_wf in H; et.
+        rewrite URA.add_comm in H. eapply URA.wf_mon; et.
+      }
+      { 
+        iIntros "H". iPoseProof (H1 with "H") as "H". et.
+      }
+      i. des.
+      eapply IH; et.
+      {
+        clear IH.
+        iIntros "H". iPoseProof (FMR0 with "H") as "H".
+        rewrite <- URA.add_assoc. iMod "H". iDestruct "H" as "[H H0]".
+        r_solve. rewrite <- URA.add_assoc. iSplitL "H"; et.
+        iPoseProof (H with "H") as "H". iMod "H".
+        iDestruct "H" as "[H H0]". iSplitL "H0"; et.  				
+      }
+    - steps. rewrite interp_hp_Guarantee.
+      unfold handle_Guarantee, mget, mput, guarantee. steps.
+      hexploit CUR. i.
+      apply iProp_sepconj in H.
+      des. rename rq into fmr0.
+      force_l.
+      instantiate (1:= (rp, fr_tgt, fmr0 ⋅ mr_tgt)).
+      steps. force_l.
+      {
+        iIntros "H". 
+        iPoseProof (FMR0 with "H") as "H". iMod "H".
+        rewrite <- URA.add_assoc.
+        iDestruct "H" as "[H H0]". 
+        iPoseProof (H with "H") as "H". iMod "H".
+        replace (rp ⋅ fr_tgt ⋅ (fmr0 ⋅ mr_tgt)) with (rp ⋅ fmr0 ⋅ (fr_tgt ⋅ mr_tgt)). 2: { r_solve. }
+        iSplitL "H"; et.
+      }
+      steps. force_l; et.
+      steps.
+      hexploit (K fmr0); et.
+      {
+        eapply own_ctx in FMR0. rewrite URA.add_assoc in FMR0. eapply own_wf in FMR0; et.
+        replace (ctx ⋅ (fmr ⋅ fr_tgt ⋅ mr_tgt)) with (ctx ⋅ fr_tgt ⋅ mr_tgt ⋅ fmr) in FMR0; r_solve.
+        eapply own_ctx, own_wf in H; et.
+        rewrite URA.add_assoc in H.
+        eapply URA.wf_mon. rewrite URA.add_comm. et.
+      }
+      {
+        iIntros "H". iPoseProof (H1 with "H") as "H". et.	
+      }
+      i. des.
+      unfold interp_hp_fun, handle_Guarantee, mget, mput in *. rewrite <- ! bind_bind in *.
+      eapply IH; et.
+      {
+        replace (fr_tgt ⋅ (fmr0 ⋅ mr_tgt)) with (fmr0 ⋅ fr_tgt ⋅ mr_tgt); r_solve.
+        et.
+      }
+      {
+        clear IH. 
+        eapply own_ctx in FMR0. rewrite URA.add_assoc in FMR0. eapply own_wf in FMR0; et.
+        replace (ctx ⋅ (fmr ⋅ fr_tgt ⋅ mr_tgt)) with (ctx ⋅ fr_tgt ⋅ mr_tgt ⋅ fmr) in FMR0; r_solve.
+        eapply own_ctx, own_wf in H; et.
+        replace (ctx ⋅ fr_tgt ⋅ mr_tgt ⋅ (rp ⋅ fmr0)) with (ctx ⋅ fr_tgt ⋅ fmr0 ⋅ mr_tgt ⋅ rp) in H; r_solve.
+        eapply URA.wf_mon; et.
+      }
+    - steps. rewrite interp_hp_Guarantee. unfold handle_Guarantee, mget, mput, guarantee. steps. 
+      unfold interp_hp_fun, handle_Guarantee, mget, mput in *. rewrite <- ! bind_bind in *.			
+      hexploit (K (c0 ⋅ fmr)). 
+      {
+        eapply own_ctx in FMR0. rewrite URA.add_assoc in FMR0. eapply own_wf in FMR0; et.
+        rewrite <- URA.add_assoc in FMR0. rewrite URA.add_assoc in FMR0.
+        eapply own_ctx, own_wf in x; et.
+        replace (ctx ⋅ fmr ⋅ (c0 ⋅ c1 ⋅ c)) with (c0 ⋅ fmr ⋅ (ctx ⋅ c1 ⋅ c)) in x; r_solve.
+        eapply URA.wf_mon; et.
+      }
+      { 
+        iIntros "[H H0]".
+        iPoseProof (x0 with "H") as "H".
+        iPoseProof (CUR with "H0") as "H0".
+        iSplitL "H"; et. 	
+      } 
+      i. des.
+      eapply IH; et.
+      {
+        iIntros "H".
+        iPoseProof (FMR0 with "H") as "H". iMod "H".
+        rewrite <- URA.add_assoc. 
+        iDestruct "H" as "[H H0]".
+        iPoseProof (x with "H0") as "H0". iMod "H0".
+        replace (c0 ⋅ fmr ⋅ c1 ⋅ c) with (fmr ⋅ (c0 ⋅ c1 ⋅ c)). 2: { r_solve. }
+        iSplitL "H"; et.
+      }
+    - gstep. econs. gfinal. left. eapply CIH; et. 
+  Admitted.
 
 
 
